@prefix : <http://purl.obolibrary.org/obo/cro.owl#> .
@prefix owl: <http://www.w3.org/2002/07/owl#> .
@prefix rdf: <http://www.w3.org/1999/02/22-rdf-syntax-ns#> .
@prefix xml: <http://www.w3.org/XML/1998/namespace> .
@prefix xsd: <http://www.w3.org/2001/XMLSchema#> .
@prefix rdfs: <http://www.w3.org/2000/01/rdf-schema#> .
@base <http://purl.obolibrary.org/obo/cro.owl> .

<http://purl.obolibrary.org/obo/cro.owl> rdf:type owl:Ontology ;
                                          owl:versionIRI <http://purl.obolibrary.org/obo/cro/releases/2019-12-11/cro.owl> ;
                                          owl:imports <http://purl.obolibrary.org/obo/cro/imports/credit_import.owl> ,
                                                      <http://purl.obolibrary.org/obo/cro/imports/iao_import.owl> ,
                                                      <http://purl.obolibrary.org/obo/cro/imports/bfo_import.owl> ;
                                          rdfs:comment "Contributor Role Ontology" .

#################################################################
#    Annotation properties
#################################################################

###  http://purl.obolibrary.org/obo/IAO_0000234
<http://purl.obolibrary.org/obo/IAO_0000234> rdf:type owl:AnnotationProperty ;
                                             rdfs:label "ontology term requester" .


###  http://purl.obolibrary.org/obo/IAO_0000412
<http://purl.obolibrary.org/obo/IAO_0000412> rdf:type owl:AnnotationProperty .


###  http://purl.obolibrary.org/obo/IAO_0100001
<http://purl.obolibrary.org/obo/IAO_0100001> rdf:type owl:AnnotationProperty ;
                                             rdfs:label "term replaced by" .


###  http://purl.org/dc/elements/1.1/creator
<http://purl.org/dc/elements/1.1/creator> rdf:type owl:AnnotationProperty .


###  http://purl.org/dc/elements/1.1/date
<http://purl.org/dc/elements/1.1/date> rdf:type owl:AnnotationProperty .


###  http://www.geneontology.org/formats/oboInOwl#created_by
<http://www.geneontology.org/formats/oboInOwl#created_by> rdf:type owl:AnnotationProperty .


###  http://www.geneontology.org/formats/oboInOwl#hasSynonym
<http://www.geneontology.org/formats/oboInOwl#hasSynonym> rdf:type owl:AnnotationProperty .


#################################################################
#    Classes
#################################################################

###  http://purl.obolibrary.org/obo/BFO_0000001
<http://purl.obolibrary.org/obo/BFO_0000001> rdfs:subClassOf owl:Thing .


###  http://purl.obolibrary.org/obo/BFO_0000002
<http://purl.obolibrary.org/obo/BFO_0000002> rdfs:subClassOf <http://purl.obolibrary.org/obo/BFO_0000001> .


###  http://purl.obolibrary.org/obo/BFO_0000020
<http://purl.obolibrary.org/obo/BFO_0000020> rdfs:subClassOf <http://purl.obolibrary.org/obo/BFO_0000002> .


###  http://purl.obolibrary.org/obo/BFO_0000031
<http://purl.obolibrary.org/obo/BFO_0000031> rdfs:subClassOf <http://purl.obolibrary.org/obo/BFO_0000002> .


###  http://purl.obolibrary.org/obo/CRO_0000000
<http://purl.obolibrary.org/obo/CRO_0000000> rdf:type owl:Class ;
                                             rdfs:subClassOf owl:Thing ;
                                             <http://purl.obolibrary.org/obo/IAO_0000111> "contributor role" ;
                                             <http://purl.obolibrary.org/obo/IAO_0000114> "http://purl.obolibrary.org/obo/IAO_0000120" ;
                                             <http://purl.obolibrary.org/obo/IAO_0000115> "A high-level classification of the diverse roles performed in the work leading to a published research output in the sciences. Its purpose to provide transparency in contributions to scholarly published work, to enable improved systems of attribution, credit, and accountability." ;
                                             <http://purl.obolibrary.org/obo/IAO_0000117> "https://orcid.org/0000-0001-5059-4132" ;
                                             <http://purl.obolibrary.org/obo/IAO_0000119> "http://dictionary.casrai.org/Contributor_Roles" ;
                                             <http://www.geneontology.org/formats/oboInOwl#hasDbXref> "9dbb95f4-55ed-4e43-9301-a9f0e3e17afe" ;
                                             <http://www.geneontology.org/formats/oboInOwl#hasSynonym> <http://purl.org/credit/ontology#CREDIT_00000000> ;
                                             rdfs:label "contributor role"@en .


###  http://purl.obolibrary.org/obo/CRO_0000001
<http://purl.obolibrary.org/obo/CRO_0000001> rdf:type owl:Class ;
                                             rdfs:subClassOf <http://purl.obolibrary.org/obo/CRO_0000000> ;
                                             <http://purl.obolibrary.org/obo/IAO_0000115> "Creation and/or presentation of a published research object, such as books, journal articles, and other publications like technical documentation, web sites, code, ontologies, or data models." ;
                                             <http://purl.obolibrary.org/obo/IAO_0000118> "writer role" ;
                                             <http://purl.org/dc/elements/1.1/creator> <http://orcid.org/0000-0001-5208-3432> ;
                                             <http://purl.org/dc/elements/1.1/date> "2018-09-14T19:47:01Z"^^xsd:dateTime ;
                                             rdfs:label "author role" .

[ rdf:type owl:Axiom ;
   owl:annotatedSource <http://purl.obolibrary.org/obo/CRO_0000001> ;
   owl:annotatedProperty <http://purl.obolibrary.org/obo/IAO_0000115> ;
   owl:annotatedTarget "Creation and/or presentation of a published research object, such as books, journal articles, and other publications like technical documentation, web sites, code, ontologies, or data models." ;
   <http://purl.obolibrary.org/obo/IAO_0000119> "https://orcid.org/0000-0002-1048-5019"
 ] .


###  http://purl.obolibrary.org/obo/CRO_0000003
<http://purl.obolibrary.org/obo/CRO_0000003> rdf:type owl:Class ;
                                             rdfs:subClassOf <http://purl.org/credit/ontology#CREDIT_00000012> ;
                                             <http://purl.obolibrary.org/obo/IAO_0000115> "Preparation, creation and/or presentation of figures for a manuscript, presentation or other use." ;
                                             <http://purl.org/dc/elements/1.1/creator> <http://orcid.org/0000-0001-5208-3432> ;
                                             <http://purl.org/dc/elements/1.1/date> "2018-09-14T19:49:22Z"^^xsd:dateTime ;
                                             rdfs:label "figure development role" .

[ rdf:type owl:Axiom ;
   owl:annotatedSource <http://purl.obolibrary.org/obo/CRO_0000003> ;
   owl:annotatedProperty <http://purl.obolibrary.org/obo/IAO_0000115> ;
   owl:annotatedTarget "Preparation, creation and/or presentation of figures for a manuscript, presentation or other use." ;
   <http://purl.obolibrary.org/obo/IAO_0000119> "http://dictionary.casrai.org/Contributor_Roles/Visualization"
 ] .


###  http://purl.obolibrary.org/obo/CRO_0000004
<http://purl.obolibrary.org/obo/CRO_0000004> rdf:type owl:Class ;
                                             rdfs:subClassOf <http://purl.org/credit/ontology#CREDIT_00000008> ;
                                             <http://purl.obolibrary.org/obo/IAO_0000115> "Translating words or text from one language to another." ;
                                             <http://purl.org/dc/elements/1.1/creator> <http://orcid.org/0000-0001-5208-3432> ;
                                             <http://purl.org/dc/elements/1.1/date> "2018-09-14T19:49:51Z"^^xsd:dateTime ;
                                             rdfs:label "translator role" .


###  http://purl.obolibrary.org/obo/CRO_0000006
<http://purl.obolibrary.org/obo/CRO_0000006> rdf:type owl:Class ;
                                             rdfs:subClassOf <http://purl.obolibrary.org/obo/CRO_0000111> ;
                                             <http://purl.obolibrary.org/obo/IAO_0000115> "Includes literature searches and contributions to review activities (systematic reviews, scoping reviews, etc.)" ;
                                             <http://purl.org/dc/elements/1.1/creator> <http://orcid.org/0000-0001-5208-3432> ;
                                             <http://purl.org/dc/elements/1.1/date> "2018-09-14T19:51:01Z"^^xsd:dateTime ;
                                             rdfs:label "background and literature search role" .


###  http://purl.obolibrary.org/obo/CRO_0000007
<http://purl.obolibrary.org/obo/CRO_0000007> rdf:type owl:Class ;
                                             rdfs:subClassOf <http://purl.obolibrary.org/obo/CRO_0000000> ;
                                             <http://purl.obolibrary.org/obo/IAO_0000115> "Coordination of research dissemination through popular media and the press, as well as community outreach and liaising of project directly to the community." ;
                                             <http://purl.obolibrary.org/obo/IAO_0000116> "Similar to vivo:OutreachProviderRole?" ;
                                             <http://purl.obolibrary.org/obo/IAO_0000118> "communication role" ,
                                                                                          "outreach role" ;
                                             <http://purl.org/dc/elements/1.1/creator> <http://orcid.org/0000-0001-5208-3432> ;
                                             <http://purl.org/dc/elements/1.1/date> "2018-09-14T19:51:26Z"^^xsd:dateTime ;
                                             rdfs:label "marketing and communication role" .


###  http://purl.obolibrary.org/obo/CRO_0000008
<http://purl.obolibrary.org/obo/CRO_0000008> rdf:type owl:Class ;
                                             rdfs:subClassOf <http://purl.obolibrary.org/obo/CRO_0000007> ;
                                             <http://purl.obolibrary.org/obo/IAO_0000115> "Creation or refinement of a website, a set of related web pages served from a single web domain." ;
                                             <http://purl.obolibrary.org/obo/IAO_0000118> "website development role" ,
                                                                                          "website maintenance role" ;
                                             <http://purl.org/dc/elements/1.1/creator> <http://orcid.org/0000-0001-5208-3432> ;
                                             <http://purl.org/dc/elements/1.1/date> "2018-09-14T19:51:53Z"^^xsd:dateTime ;
                                             rdfs:label "website role" .

[ rdf:type owl:Axiom ;
   owl:annotatedSource <http://purl.obolibrary.org/obo/CRO_0000008> ;
   owl:annotatedProperty <http://purl.obolibrary.org/obo/IAO_0000115> ;
   owl:annotatedTarget "Creation or refinement of a website, a set of related web pages served from a single web domain." ;
   <http://purl.obolibrary.org/obo/IAO_0000119> "https://www.wikidata.org/wiki/Q35127"
 ] .


###  http://purl.obolibrary.org/obo/CRO_0000009
<http://purl.obolibrary.org/obo/CRO_0000009> rdf:type owl:Class ;
                                             rdfs:subClassOf owl:Thing ;
                                             <http://purl.obolibrary.org/obo/IAO_0000115> "A communication role that encompasses facilitate co-operation between people or organizations." ;
                                             <http://purl.org/dc/elements/1.1/creator> <http://orcid.org/0000-0001-5208-3432> ;
                                             <http://purl.org/dc/elements/1.1/date> "2018-09-14T19:52:02Z"^^xsd:dateTime ;
                                             rdfs:label "obsolete networking facilitation role" ;
                                             owl:deprecated "true"^^xsd:boolean .

[ rdf:type owl:Axiom ;
   owl:annotatedSource <http://purl.obolibrary.org/obo/CRO_0000009> ;
   owl:annotatedProperty <http://purl.obolibrary.org/obo/IAO_0000115> ;
   owl:annotatedTarget "A communication role that encompasses facilitate co-operation between people or organizations." ;
   <http://purl.obolibrary.org/obo/IAO_0000119> "(2009) The functions and roles of network facilitators. In: Franz HW., Sarcina R. (eds) Building Leadership in Project and Network Management. Springer, Berlin, Heidelberg"
 ] .


###  http://purl.obolibrary.org/obo/CRO_0000010
<http://purl.obolibrary.org/obo/CRO_0000010> rdf:type owl:Class ;
                                             rdfs:subClassOf owl:Thing ;
                                             <http://purl.obolibrary.org/obo/IAO_0000115> "A communication role that involves the activity, set of institutions, and processes for creating, communicating, delivering, and exchanging offerings that have value for customers, clients, partners, and society at large." ;
                                             <http://purl.org/dc/elements/1.1/creator> <http://orcid.org/0000-0001-5208-3432> ;
                                             <http://purl.org/dc/elements/1.1/date> "2018-09-14T19:52:12Z"^^xsd:dateTime ;
                                             rdfs:label "obsolete marketing role" ;
                                             owl:deprecated "true"^^xsd:boolean .

[ rdf:type owl:Axiom ;
   owl:annotatedSource <http://purl.obolibrary.org/obo/CRO_0000010> ;
   owl:annotatedProperty <http://purl.obolibrary.org/obo/IAO_0000115> ;
   owl:annotatedTarget "A communication role that involves the activity, set of institutions, and processes for creating, communicating, delivering, and exchanging offerings that have value for customers, clients, partners, and society at large." ;
   <http://purl.obolibrary.org/obo/IAO_0000119> "https://www.ama.org/the-definition-of-marketing/"
 ] .


###  http://purl.obolibrary.org/obo/CRO_0000011
<http://purl.obolibrary.org/obo/CRO_0000011> rdf:type owl:Class ;
                                             rdfs:subClassOf <http://purl.obolibrary.org/obo/CRO_0000007> ;
                                             <http://purl.obolibrary.org/obo/IAO_0000115> "A communication role in which one records the details of an event, a process, a workflow, etc." ;
                                             <http://purl.org/dc/elements/1.1/creator> <http://orcid.org/0000-0001-5208-3432> ;
                                             <http://purl.org/dc/elements/1.1/date> "2018-09-14T19:52:17Z"^^xsd:dateTime ;
                                             rdfs:label "documentation role" .

[ rdf:type owl:Axiom ;
   owl:annotatedSource <http://purl.obolibrary.org/obo/CRO_0000011> ;
   owl:annotatedProperty <http://purl.obolibrary.org/obo/IAO_0000115> ;
   owl:annotatedTarget "A communication role in which one records the details of an event, a process, a workflow, etc." ;
   <http://purl.obolibrary.org/obo/IAO_0000119> "https://dictionary.cambridge.org/us/dictionary/english/document"
 ] .


###  http://purl.obolibrary.org/obo/CRO_0000012
<http://purl.obolibrary.org/obo/CRO_0000012> rdf:type owl:Class ;
                                             rdfs:subClassOf <http://purl.org/credit/ontology#CREDIT_00000012> ;
                                             <http://purl.obolibrary.org/obo/IAO_0000115> "A communication role that utilizes the art or profession of using design elements (such as typography and images) to convey information, create visualizations, or create an effect." ;
                                             <http://purl.org/dc/elements/1.1/creator> <http://orcid.org/0000-0001-5208-3432> ;
                                             <http://purl.org/dc/elements/1.1/date> "2018-09-14T19:52:27Z"^^xsd:dateTime ;
                                             rdfs:label "graphic design role" .

[ rdf:type owl:Axiom ;
   owl:annotatedSource <http://purl.obolibrary.org/obo/CRO_0000012> ;
   owl:annotatedProperty <http://purl.obolibrary.org/obo/IAO_0000115> ;
   owl:annotatedTarget "A communication role that utilizes the art or profession of using design elements (such as typography and images) to convey information, create visualizations, or create an effect." ;
   <http://purl.obolibrary.org/obo/IAO_0000119> "https://www.merriam-webster.com/dictionary/graphic%20design"
 ] .


###  http://purl.obolibrary.org/obo/CRO_0000014
<http://purl.obolibrary.org/obo/CRO_0000014> rdf:type owl:Class ;
                                             rdfs:subClassOf <http://purl.obolibrary.org/obo/CRO_0000001> ;
                                             <http://purl.obolibrary.org/obo/IAO_0000115> "Creation of software documentation." ;
                                             <http://purl.obolibrary.org/obo/IAO_0000118> "software documentation role" ;
                                             <http://purl.org/dc/elements/1.1/creator> <http://orcid.org/0000-0001-5208-3432> ;
                                             <http://purl.org/dc/elements/1.1/date> "2018-09-14T20:26:05Z"^^xsd:dateTime ;
                                             rdfs:label "technical documentation role" .


###  http://purl.obolibrary.org/obo/CRO_0000015
<http://purl.obolibrary.org/obo/CRO_0000015> rdf:type owl:Class ;
                                             rdfs:subClassOf <http://purl.obolibrary.org/obo/CRO_0000000> ;
                                             <http://purl.obolibrary.org/obo/IAO_0000115> "A role that encompasses effective and efficient operation and usage of data, including, but not limited to management, handling, or manipulation." ;
                                             <http://purl.org/dc/elements/1.1/creator> <http://orcid.org/0000-0001-5208-3432> ;
                                             <http://purl.org/dc/elements/1.1/date> "2018-09-14T19:55:34Z"^^xsd:dateTime ;
                                             rdfs:label "data role" .


###  http://purl.obolibrary.org/obo/CRO_0000016
<http://purl.obolibrary.org/obo/CRO_0000016> rdf:type owl:Class ;
                                             rdfs:subClassOf <http://purl.obolibrary.org/obo/CRO_0000000> ;
                                             <http://purl.obolibrary.org/obo/IAO_0000115> "A role in which a person participates in the transfer of knowledge and skills, through teaching, development of educational materials or curriculum, through program development or other means." ;
                                             <http://purl.obolibrary.org/obo/IAO_0000118> "educational role" ;
                                             <http://purl.org/dc/elements/1.1/creator> <http://orcid.org/0000-0001-5208-3432> ;
                                             <http://purl.org/dc/elements/1.1/date> "2018-09-14T19:55:45Z"^^xsd:dateTime ;
                                             rdfs:label "education and training role" .


###  http://purl.obolibrary.org/obo/CRO_0000018
<http://purl.obolibrary.org/obo/CRO_0000018> rdf:type owl:Class ;
                                             rdfs:subClassOf owl:Thing ;
                                             <http://purl.obolibrary.org/obo/IAO_0000115> "A role that involves the development, management, and use of computer-based information systems." ;
                                             <http://purl.org/dc/elements/1.1/creator> <http://orcid.org/0000-0001-5208-3432> ;
                                             <http://purl.org/dc/elements/1.1/date> "2018-09-14T19:56:05Z"^^xsd:dateTime ;
                                             rdfs:label "obsolete information technology systems role" ;
                                             owl:deprecated "true"^^xsd:boolean .

[ rdf:type owl:Axiom ;
   owl:annotatedSource <http://purl.obolibrary.org/obo/CRO_0000018> ;
   owl:annotatedProperty <http://purl.obolibrary.org/obo/IAO_0000115> ;
   owl:annotatedTarget "A role that involves the development, management, and use of computer-based information systems." ;
   <http://purl.obolibrary.org/obo/IAO_0000119> "https://www.wikidata.org/wiki/Q11661"
 ] .


###  http://purl.obolibrary.org/obo/CRO_0000019
<http://purl.obolibrary.org/obo/CRO_0000019> rdf:type owl:Class ;
                                             rdfs:subClassOf <http://purl.org/credit/ontology#CREDIT_00000009> ;
                                             <http://purl.obolibrary.org/obo/IAO_0000115> "Verification that software meets requirements; validation that software meets users' needs, identification of software bugs, assessment of software performance and usability." ;
                                             <http://purl.obolibrary.org/obo/IAO_0000118> "Software Quality Assurance Role" ;
                                             <http://purl.org/dc/elements/1.1/creator> <http://orcid.org/0000-0001-5208-3432> ;
                                             <http://purl.org/dc/elements/1.1/date> "2018-09-14T20:26:00Z"^^xsd:dateTime ;
                                             rdfs:label "software testing role" .


###  http://purl.obolibrary.org/obo/CRO_0000020
<http://purl.obolibrary.org/obo/CRO_0000020> rdf:type owl:Class ;
                                             rdfs:subClassOf <http://purl.obolibrary.org/obo/CRO_0000078> ;
                                             <http://purl.obolibrary.org/obo/IAO_0000115> "A role related to creations of the mind, such as inventions; literary and artistic works; designs; and symbols, names and images used in commerce. from." ;
                                             <http://purl.org/dc/elements/1.1/creator> <http://orcid.org/0000-0001-5208-3432> ;
                                             <http://purl.org/dc/elements/1.1/date> "2018-09-14T19:56:34Z"^^xsd:dateTime ;
                                             rdfs:label "intellectual property role" .

[ rdf:type owl:Axiom ;
   owl:annotatedSource <http://purl.obolibrary.org/obo/CRO_0000020> ;
   owl:annotatedProperty <http://purl.obolibrary.org/obo/IAO_0000115> ;
   owl:annotatedTarget "A role related to creations of the mind, such as inventions; literary and artistic works; designs; and symbols, names and images used in commerce. from." ;
   <http://purl.obolibrary.org/obo/IAO_0000119> "https://www.wipo.int/about-ip/en/"
 ] .


###  http://purl.obolibrary.org/obo/CRO_0000022
<http://purl.obolibrary.org/obo/CRO_0000022> rdf:type owl:Class ;
                                             rdfs:subClassOf <http://purl.obolibrary.org/obo/CRO_0000000> ;
                                             <http://purl.obolibrary.org/obo/IAO_0000115> "Policy development generally involves research, analysis, consultation and synthesis of information to produce recommendations for action by an individual or an organization. It should also involve an evaluation of options against a set of criteria used to assess each option." ;
                                             <http://purl.org/dc/elements/1.1/creator> <http://orcid.org/0000-0001-5208-3432> ;
                                             <http://purl.org/dc/elements/1.1/date> "2018-09-14T20:04:29Z"^^xsd:dateTime ;
                                             rdfs:label "policy development role" .


###  http://purl.obolibrary.org/obo/CRO_0000023
<http://purl.obolibrary.org/obo/CRO_0000023> rdf:type owl:Class ;
                                             rdfs:subClassOf <http://purl.obolibrary.org/obo/CRO_0000000> ;
                                             <http://purl.obolibrary.org/obo/IAO_0000115> "Set of activities aimed at prolonging the life of a record." ;
                                             <http://purl.org/dc/elements/1.1/creator> <http://orcid.org/0000-0001-5208-3432> ;
                                             <http://purl.org/dc/elements/1.1/date> "2018-09-14T20:04:39Z"^^xsd:dateTime ;
                                             rdfs:label "preservation role" .

[ rdf:type owl:Axiom ;
   owl:annotatedSource <http://purl.obolibrary.org/obo/CRO_0000023> ;
   owl:annotatedProperty <http://purl.obolibrary.org/obo/IAO_0000115> ;
   owl:annotatedTarget "Set of activities aimed at prolonging the life of a record." ;
   <http://purl.obolibrary.org/obo/IAO_0000119> "https://www.wikidata.org/wiki/Q830393"
 ] .


###  http://purl.obolibrary.org/obo/CRO_0000025
<http://purl.obolibrary.org/obo/CRO_0000025> rdf:type owl:Class ;
                                             rdfs:subClassOf <http://purl.obolibrary.org/obo/CRO_0000078> ;
                                             <http://purl.obolibrary.org/obo/IAO_0000115> "Manage regulatory and compliance issues for the research project." ;
                                             <http://purl.obolibrary.org/obo/IAO_0000118> "regulatory administration role" ;
                                             <http://purl.org/dc/elements/1.1/creator> <http://orcid.org/0000-0001-5208-3432> ;
                                             <http://purl.org/dc/elements/1.1/date> "2018-09-14T20:05:56Z"^^xsd:dateTime ;
                                             rdfs:label "regulatory and compliance role" .


###  http://purl.obolibrary.org/obo/CRO_0000026
<http://purl.obolibrary.org/obo/CRO_0000026> rdf:type owl:Class ;
                                             rdfs:subClassOf <http://purl.obolibrary.org/obo/CRO_0000000> ;
                                             <http://purl.obolibrary.org/obo/IAO_0000115> "A person that is responsible for usage of instrumentation, such as equipment or devices, or instruments like a survey or questionnaire." ;
                                             <http://purl.org/dc/elements/1.1/creator> <http://orcid.org/0000-0001-5208-3432> ;
                                             <http://purl.org/dc/elements/1.1/date> "2018-09-14T20:06:00Z"^^xsd:dateTime ;
                                             rdfs:label "instrumentation role" .


###  http://purl.obolibrary.org/obo/CRO_0000027
<http://purl.obolibrary.org/obo/CRO_0000027> rdf:type owl:Class ;
                                             rdfs:subClassOf <http://purl.obolibrary.org/obo/CRO_0000023> ;
                                             <http://purl.obolibrary.org/obo/IAO_0000115> "Management activities to annotate, maintain, research, and preserve physical objects to maximize their use for research and education now and into the future." ;
                                             <http://purl.obolibrary.org/obo/IAO_0000234> "https://orcid.org/0000-0002-2908-3327" ;
                                             <http://purl.org/dc/elements/1.1/creator> <http://orcid.org/0000-0001-5208-3432> ;
                                             rdfs:label "curator role" .


###  http://purl.obolibrary.org/obo/CRO_0000028
<http://purl.obolibrary.org/obo/CRO_0000028> rdf:type owl:Class ;
                                             rdfs:subClassOf <http://purl.obolibrary.org/obo/CRO_0000000> ;
                                             <http://purl.obolibrary.org/obo/IAO_0000115> "Activities to obtain physical objects for research or scholarly purposes or to add to a collection." ;
                                             <http://purl.obolibrary.org/obo/IAO_0000234> "https://orcid.org/0000-0002-2908-3327" ;
                                             <http://purl.org/dc/elements/1.1/creator> <http://orcid.org/0000-0001-5208-3432> ;
                                             rdfs:label "collection role" .


###  http://purl.obolibrary.org/obo/CRO_0000031
<http://purl.obolibrary.org/obo/CRO_0000031> rdf:type owl:Class ;
                                             rdfs:subClassOf <http://purl.obolibrary.org/obo/CRO_0000078> ;
                                             <http://purl.obolibrary.org/obo/IAO_0000115> "Coordination of diverse team members, often across different disciplines and locations." ;
                                             <http://purl.org/dc/elements/1.1/creator> <http://orcid.org/0000-0001-5208-3432> ;
                                             <http://purl.org/dc/elements/1.1/date> "2018-09-14T20:06:26Z"^^xsd:dateTime ;
                                             rdfs:label "team management role" .


###  http://purl.obolibrary.org/obo/CRO_0000033
<http://purl.obolibrary.org/obo/CRO_0000033> rdf:type owl:Class ;
                                             rdfs:subClassOf owl:Thing ;
                                             <http://purl.obolibrary.org/obo/IAO_0000115> "The compiling of information with intent to prepare combined datasets for data processing." ;
                                             <http://purl.obolibrary.org/obo/IAO_0100001> <http://purl.obolibrary.org/obo/CRO_0000036> ;
                                             <http://purl.org/dc/elements/1.1/creator> <http://orcid.org/0000-0001-5208-3432> ;
                                             <http://purl.org/dc/elements/1.1/date> "2018-09-14T20:11:23Z"^^xsd:dateTime ;
                                             rdfs:label "obsolete data aggregation role" ;
                                             owl:deprecated "true"^^xsd:boolean .

[ rdf:type owl:Axiom ;
   owl:annotatedSource <http://purl.obolibrary.org/obo/CRO_0000033> ;
   owl:annotatedProperty <http://purl.obolibrary.org/obo/IAO_0000115> ;
   owl:annotatedTarget "The compiling of information with intent to prepare combined datasets for data processing." ;
   <http://purl.obolibrary.org/obo/IAO_0000119> "Stanley, Jay; Steinhardt, Barry (January 2003). \"Bigger Monster, Weaker Chains: The Growth of an American Surveillance Society\". American Civil Liberties Union."
 ] .


###  http://purl.obolibrary.org/obo/CRO_0000035
<http://purl.obolibrary.org/obo/CRO_0000035> rdf:type owl:Class ;
                                             rdfs:subClassOf <http://purl.org/credit/ontology#CREDIT_00000003> ;
                                             <http://purl.obolibrary.org/obo/IAO_0000115> "Statistical aspects of research, including data collection, organization, analysis, interpretation and presentation of data from surveys and experiments" ;
                                             <http://purl.obolibrary.org/obo/IAO_0000118> "statistical data analysis role" ;
                                             <http://purl.org/dc/elements/1.1/creator> <http://orcid.org/0000-0001-5208-3432> ;
                                             <http://purl.org/dc/elements/1.1/date> "2018-09-14T20:11:35Z"^^xsd:dateTime ;
                                             rdfs:label "statistical analysis role" .

[ rdf:type owl:Axiom ;
   owl:annotatedSource <http://purl.obolibrary.org/obo/CRO_0000035> ;
   owl:annotatedProperty <http://purl.obolibrary.org/obo/IAO_0000115> ;
   owl:annotatedTarget "Statistical aspects of research, including data collection, organization, analysis, interpretation and presentation of data from surveys and experiments" ;
   <http://purl.obolibrary.org/obo/IAO_0000119> "https://en.wikipedia.org/wiki/Statistics"
 ] .


###  http://purl.obolibrary.org/obo/CRO_0000036
<http://purl.obolibrary.org/obo/CRO_0000036> rdf:type owl:Class ;
                                             rdfs:subClassOf <http://purl.obolibrary.org/obo/CRO_0000015> ;
                                             <http://purl.obolibrary.org/obo/IAO_0000115> "The process of gathering and measuring data, information or any variables of interest in a standardized and established manner that enables the collector to answer or test hypothesis and evaluate outcomes of the particular collection." ;
                                             <http://purl.obolibrary.org/obo/IAO_0000118> "data aggregation role" ;
                                             <http://purl.org/dc/elements/1.1/creator> <http://orcid.org/0000-0001-5208-3432> ;
                                             <http://purl.org/dc/elements/1.1/date> "2018-09-14T20:11:40Z"^^xsd:dateTime ;
                                             rdfs:label "data collection role" .

[ rdf:type owl:Axiom ;
   owl:annotatedSource <http://purl.obolibrary.org/obo/CRO_0000036> ;
   owl:annotatedProperty <http://purl.obolibrary.org/obo/IAO_0000115> ;
   owl:annotatedTarget "The process of gathering and measuring data, information or any variables of interest in a standardized and established manner that enables the collector to answer or test hypothesis and evaluate outcomes of the particular collection." ;
   <http://purl.obolibrary.org/obo/IAO_0000119> "https://www.techopedia.com/definition/30318/data-collection"
 ] .


###  http://purl.obolibrary.org/obo/CRO_0000038
<http://purl.obolibrary.org/obo/CRO_0000038> rdf:type owl:Class ;
                                             rdfs:subClassOf <http://purl.obolibrary.org/obo/CRO_0000015> ;
                                             <http://purl.obolibrary.org/obo/IAO_0000115> "The annotation of data with descriptive information that describes the data (metadata), with the goal of making the data more usuable or reusable for future use." ;
                                             <http://purl.obolibrary.org/obo/IAO_0000118> "metadata application role" ;
                                             <http://purl.org/dc/elements/1.1/creator> <http://orcid.org/0000-0001-5208-3432> ;
                                             <http://purl.org/dc/elements/1.1/date> "2018-09-14T20:11:50Z"^^xsd:dateTime ;
                                             rdfs:label "metadata role" .

[ rdf:type owl:Axiom ;
   owl:annotatedSource <http://purl.obolibrary.org/obo/CRO_0000038> ;
   owl:annotatedProperty <http://purl.obolibrary.org/obo/IAO_0000115> ;
   owl:annotatedTarget "The annotation of data with descriptive information that describes the data (metadata), with the goal of making the data more usuable or reusable for future use." ;
   <http://purl.obolibrary.org/obo/IAO_0000119> "https://whatis.techtarget.com/definition/metadata-management"
 ] .


###  http://purl.obolibrary.org/obo/CRO_0000039
<http://purl.obolibrary.org/obo/CRO_0000039> rdf:type owl:Class ;
                                             rdfs:subClassOf <http://purl.obolibrary.org/obo/CRO_0000015> ;
                                             <http://purl.obolibrary.org/obo/IAO_0000115> "The process of inputting data into a computerized form." ;
                                             <http://purl.org/dc/elements/1.1/creator> <http://orcid.org/0000-0001-5208-3432> ;
                                             <http://purl.org/dc/elements/1.1/date> "2018-09-14T20:11:54Z"^^xsd:dateTime ;
                                             rdfs:label "data entry role" .

[ rdf:type owl:Axiom ;
   owl:annotatedSource <http://purl.obolibrary.org/obo/CRO_0000039> ;
   owl:annotatedProperty <http://purl.obolibrary.org/obo/IAO_0000115> ;
   owl:annotatedTarget "The process of inputting data into a computerized form." ;
   <http://purl.obolibrary.org/obo/IAO_0000119> "https://www.dictionary.com/browse/data-entry"
 ] .


###  http://purl.obolibrary.org/obo/CRO_0000040
<http://purl.obolibrary.org/obo/CRO_0000040> rdf:type owl:Class ;
                                             rdfs:subClassOf <http://purl.obolibrary.org/obo/CRO_0000015> ;
                                             <http://purl.obolibrary.org/obo/IAO_0000115> "The process of combining data from different sources to provide a standardized or unified view." ;
                                             <http://purl.org/dc/elements/1.1/creator> <http://orcid.org/0000-0001-5208-3432> ;
                                             <http://purl.org/dc/elements/1.1/date> "2018-09-14T20:12:00Z"^^xsd:dateTime ;
                                             rdfs:label "data integration role" .

[ rdf:type owl:Axiom ;
   owl:annotatedSource <http://purl.obolibrary.org/obo/CRO_0000040> ;
   owl:annotatedProperty <http://purl.obolibrary.org/obo/IAO_0000115> ;
   owl:annotatedTarget "The process of combining data from different sources to provide a standardized or unified view." ;
   <http://purl.obolibrary.org/obo/IAO_0000119> "https://www.wikidata.org/wiki/Q386824"
 ] .


###  http://purl.obolibrary.org/obo/CRO_0000041
<http://purl.obolibrary.org/obo/CRO_0000041> rdf:type owl:Class ;
                                             rdfs:subClassOf <http://purl.obolibrary.org/obo/CRO_0000015> ;
                                             <http://purl.obolibrary.org/obo/IAO_0000115> "The process of creating a data model for an information system by applying certain formal techniques." ;
                                             <http://purl.org/dc/elements/1.1/creator> <http://orcid.org/0000-0001-5208-3432> ;
                                             <http://purl.org/dc/elements/1.1/date> "2018-09-14T20:12:07Z"^^xsd:dateTime ;
                                             rdfs:label "data modeling role" .

[ rdf:type owl:Axiom ;
   owl:annotatedSource <http://purl.obolibrary.org/obo/CRO_0000041> ;
   owl:annotatedProperty <http://purl.obolibrary.org/obo/IAO_0000115> ;
   owl:annotatedTarget "The process of creating a data model for an information system by applying certain formal techniques." ;
   <http://purl.obolibrary.org/obo/IAO_0000119> "https://www.wikidata.org/wiki/Q367664"
 ] .


###  http://purl.obolibrary.org/obo/CRO_0000042
<http://purl.obolibrary.org/obo/CRO_0000042> rdf:type owl:Class ;
                                             rdfs:subClassOf <http://purl.obolibrary.org/obo/CRO_0000015> ;
                                             <http://purl.obolibrary.org/obo/IAO_0000115> "A procedure intended to verify the efficiency and reliability of data." ;
                                             <http://purl.obolibrary.org/obo/IAO_0000118> "Data Scrubbing Role" ;
                                             <http://purl.org/dc/elements/1.1/creator> <http://orcid.org/0000-0001-5208-3432> ;
                                             <http://purl.org/dc/elements/1.1/date> "2018-09-14T20:12:14Z"^^xsd:dateTime ;
                                             rdfs:label "data quality assurance role" .

[ rdf:type owl:Axiom ;
   owl:annotatedSource <http://purl.obolibrary.org/obo/CRO_0000042> ;
   owl:annotatedProperty <http://purl.obolibrary.org/obo/IAO_0000115> ;
   owl:annotatedTarget "A procedure intended to verify the efficiency and reliability of data." ;
   <http://purl.obolibrary.org/obo/IAO_0000119> "https://www.techopedia.com/definition/14653/data-quality"
 ] .


###  http://purl.obolibrary.org/obo/CRO_0000043
<http://purl.obolibrary.org/obo/CRO_0000043> rdf:type owl:Class ;
                                             rdfs:subClassOf owl:Thing ;
                                             <http://purl.obolibrary.org/obo/IAO_0000115> "The process of creating data standards, which are the rules by which data are described and recorded in order to share, exchange, and understand data. Examples include development of an ontology, terminology, code lists, etc." ;
                                             <http://purl.org/dc/elements/1.1/creator> <http://orcid.org/0000-0001-5208-3432> ;
                                             <http://purl.org/dc/elements/1.1/date> "2018-09-14T20:12:25Z"^^xsd:dateTime ;
                                             rdfs:label "obsolete data standards developer role" ;
                                             owl:deprecated "true"^^xsd:boolean .

[ rdf:type owl:Axiom ;
   owl:annotatedSource <http://purl.obolibrary.org/obo/CRO_0000043> ;
   owl:annotatedProperty <http://purl.obolibrary.org/obo/IAO_0000115> ;
   owl:annotatedTarget "The process of creating data standards, which are the rules by which data are described and recorded in order to share, exchange, and understand data. Examples include development of an ontology, terminology, code lists, etc." ;
   <http://purl.obolibrary.org/obo/IAO_0000119> "https://www.usgs.gov/products/data-and-tools/data-management/data-standards"
 ] .


###  http://purl.obolibrary.org/obo/CRO_0000045
<http://purl.obolibrary.org/obo/CRO_0000045> rdf:type owl:Class ;
                                             rdfs:subClassOf <http://purl.obolibrary.org/obo/CRO_0000016> ;
                                             <http://purl.obolibrary.org/obo/IAO_0000115> "An educational role in which a person develops educational or training materials that are intended to transfer knowledge, for use in a classroom, indpendent learning or other settings." ;
                                             <http://purl.obolibrary.org/obo/IAO_0000118> "educational material development role" ;
                                             <http://purl.org/dc/elements/1.1/creator> <http://orcid.org/0000-0001-5208-3432> ;
                                             <http://purl.org/dc/elements/1.1/date> "2018-09-14T20:15:18Z"^^xsd:dateTime ;
                                             rdfs:label "training material role" .


###  http://purl.obolibrary.org/obo/CRO_0000046
<http://purl.obolibrary.org/obo/CRO_0000046> rdf:type owl:Class ;
                                             rdfs:subClassOf <http://purl.obolibrary.org/obo/CRO_0000016> ;
                                             <http://purl.obolibrary.org/obo/IAO_0000115> "An educational role in which a person participates in the development of an educational program, designed for learners to achieve a set of compentencies around a given topic or area of focus." ;
                                             <http://purl.obolibrary.org/obo/IAO_0000118> "educational program development role" ;
                                             <http://purl.org/dc/elements/1.1/creator> <http://orcid.org/0000-0001-5208-3432> ;
                                             <http://purl.org/dc/elements/1.1/date> "2018-09-14T20:15:23Z"^^xsd:dateTime ;
                                             rdfs:label "training program development role" .


###  http://purl.obolibrary.org/obo/CRO_0000047
<http://purl.obolibrary.org/obo/CRO_0000047> rdf:type owl:Class ;
                                             rdfs:subClassOf <http://purl.obolibrary.org/obo/CRO_0000016> ;
                                             <http://purl.obolibrary.org/obo/IAO_0000115> "An educational role in which knowledge and skills are transferred through teaching." ;
                                             <http://purl.obolibrary.org/obo/IAO_0000116> "This may be equivalent to vivo:Teacher Role." ;
                                             <http://purl.obolibrary.org/obo/IAO_0000118> "educational instruction role" ,
                                                                                          "educational training role" ,
                                                                                          "teaching role" ;
                                             <http://purl.org/dc/elements/1.1/creator> <http://orcid.org/0000-0001-5208-3432> ;
                                             <http://purl.org/dc/elements/1.1/date> "2018-09-14T20:15:29Z"^^xsd:dateTime ;
                                             rdfs:label "instruction role" .

[ rdf:type owl:Axiom ;
   owl:annotatedSource <http://purl.obolibrary.org/obo/CRO_0000047> ;
   owl:annotatedProperty <http://purl.obolibrary.org/obo/IAO_0000115> ;
   owl:annotatedTarget "An educational role in which knowledge and skills are transferred through teaching." ;
   <http://purl.obolibrary.org/obo/IAO_0000119> "https://www.wikidata.org/wiki/Q8434"
 ] .


###  http://purl.obolibrary.org/obo/CRO_0000048
<http://purl.obolibrary.org/obo/CRO_0000048> rdf:type owl:Class ;
                                             rdfs:subClassOf <http://purl.obolibrary.org/obo/CRO_0000000> ;
                                             <http://purl.obolibrary.org/obo/IAO_0000115> "An information technology systems role that specifically focuses on the computer hardware, the physical components of a computer system." ;
                                             <http://purl.obolibrary.org/obo/IAO_0000118> "hardware systems role" ;
                                             <http://purl.org/dc/elements/1.1/creator> <http://orcid.org/0000-0001-5208-3432> ;
                                             <http://purl.org/dc/elements/1.1/date> "2018-09-14T20:17:16Z"^^xsd:dateTime ;
                                             rdfs:label "hardware role" .

[ rdf:type owl:Axiom ;
   owl:annotatedSource <http://purl.obolibrary.org/obo/CRO_0000048> ;
   owl:annotatedProperty <http://purl.obolibrary.org/obo/IAO_0000115> ;
   owl:annotatedTarget "An information technology systems role that specifically focuses on the computer hardware, the physical components of a computer system." ;
   <http://purl.obolibrary.org/obo/IAO_0000119> "https://www.wikidata.org/wiki/Q3966"
 ] .


###  http://purl.obolibrary.org/obo/CRO_0000049
<http://purl.obolibrary.org/obo/CRO_0000049> rdf:type owl:Class ;
                                             rdfs:subClassOf owl:Thing ;
                                             <http://purl.obolibrary.org/obo/IAO_0000115> "An information technology systems role that specifically focuses on the computer software, the non-tangible executable component of a computer." ;
                                             <http://purl.obolibrary.org/obo/IAO_0100001> <http://purl.org/credit/ontology#CREDIT_00000009> ;
                                             <http://purl.org/dc/elements/1.1/creator> <http://orcid.org/0000-0001-5208-3432> ;
                                             <http://purl.org/dc/elements/1.1/date> "2018-09-14T20:17:20Z"^^xsd:dateTime ;
                                             rdfs:label "obsolete software systems role" ;
                                             owl:deprecated "true"^^xsd:boolean .

[ rdf:type owl:Axiom ;
   owl:annotatedSource <http://purl.obolibrary.org/obo/CRO_0000049> ;
   owl:annotatedProperty <http://purl.obolibrary.org/obo/IAO_0000115> ;
   owl:annotatedTarget "An information technology systems role that specifically focuses on the computer software, the non-tangible executable component of a computer." ;
   <http://purl.obolibrary.org/obo/IAO_0000119> "https://www.wikidata.org/wiki/Q7397"
 ] .


###  http://purl.obolibrary.org/obo/CRO_0000050
<http://purl.obolibrary.org/obo/CRO_0000050> rdf:type owl:Class ;
                                             rdfs:subClassOf <http://purl.obolibrary.org/obo/CRO_0000108> ;
                                             <http://purl.obolibrary.org/obo/IAO_0000115> "A role usually within the Information Technology department, charged with the creation, maintenance, backups, querying, tuning, user rights assignment and security of an organization's databases." ;
                                             <http://purl.obolibrary.org/obo/IAO_0000118> "database administration role" ;
                                             <http://purl.org/dc/elements/1.1/creator> <http://orcid.org/0000-0001-5208-3432> ;
                                             <http://purl.org/dc/elements/1.1/date> "2018-09-14T20:17:25Z"^^xsd:dateTime ;
                                             rdfs:label "database administrator role" .

[ rdf:type owl:Axiom ;
   owl:annotatedSource <http://purl.obolibrary.org/obo/CRO_0000050> ;
   owl:annotatedProperty <http://purl.obolibrary.org/obo/IAO_0000115> ;
   owl:annotatedTarget "A role usually within the Information Technology department, charged with the creation, maintenance, backups, querying, tuning, user rights assignment and security of an organization's databases." ;
   <http://purl.obolibrary.org/obo/IAO_0000119> "https://www.techopedia.com/definition/1187/database-administrator-dba"
 ] .


###  http://purl.obolibrary.org/obo/CRO_0000051
<http://purl.obolibrary.org/obo/CRO_0000051> rdf:type owl:Class ;
                                             rdfs:subClassOf <http://purl.org/credit/ontology#CREDIT_00000009> ;
                                             <http://purl.obolibrary.org/obo/IAO_0000115> "A software systems role that involves maintenance and operation of a computer system and/or network." ;
                                             <http://purl.obolibrary.org/obo/IAO_0000118> "sysadmin role" ,
                                                                                          "systems administration role" ;
                                             <http://purl.org/dc/elements/1.1/creator> <http://orcid.org/0000-0001-5208-3432> ;
                                             <http://purl.org/dc/elements/1.1/date> "2018-09-14T20:17:32Z"^^xsd:dateTime ;
                                             rdfs:label "system administrator role" .

[ rdf:type owl:Axiom ;
   owl:annotatedSource <http://purl.obolibrary.org/obo/CRO_0000051> ;
   owl:annotatedProperty <http://purl.obolibrary.org/obo/IAO_0000115> ;
   owl:annotatedTarget "A software systems role that involves maintenance and operation of a computer system and/or network." ;
   <http://purl.obolibrary.org/obo/IAO_0000119> "https://www.wikidata.org/wiki/Q327353"
 ] .


###  http://purl.obolibrary.org/obo/CRO_0000052
<http://purl.obolibrary.org/obo/CRO_0000052> rdf:type owl:Class ;
                                             rdfs:subClassOf <http://purl.org/credit/ontology#CREDIT_00000006> ;
                                             <http://purl.obolibrary.org/obo/IAO_0000115> "A methodology role that involves development of information that suggests how something should be done." ;
                                             <http://purl.obolibrary.org/obo/IAO_0000118> "Best Practices Role" ,
                                                                                          "guideline development role" ,
                                                                                          "standard operating procedure development role" ;
                                             <http://purl.org/dc/elements/1.1/creator> <http://orcid.org/0000-0001-5208-3432> ;
                                             <http://purl.org/dc/elements/1.1/date> "2018-09-14T20:19:52Z"^^xsd:dateTime ;
                                             rdfs:label "standards role" .

[ rdf:type owl:Axiom ;
   owl:annotatedSource <http://purl.obolibrary.org/obo/CRO_0000052> ;
   owl:annotatedProperty <http://purl.obolibrary.org/obo/IAO_0000115> ;
   owl:annotatedTarget "A methodology role that involves development of information that suggests how something should be done." ;
   <http://purl.obolibrary.org/obo/IAO_0000119> "https://dictionary.cambridge.org/us/dictionary/english/guideline"
 ] .


###  http://purl.obolibrary.org/obo/CRO_0000053
<http://purl.obolibrary.org/obo/CRO_0000053> rdf:type owl:Class ;
                                             rdfs:subClassOf <http://purl.org/credit/ontology#CREDIT_00000006> ;
                                             <http://purl.obolibrary.org/obo/IAO_0000115> "A methodology role that involves creation of a detailed plan of a scientific or medical experiment, treatment, or procedure." ;
                                             <http://purl.obolibrary.org/obo/IAO_0000118> "protocol development role" ;
                                             <http://purl.org/dc/elements/1.1/creator> <http://orcid.org/0000-0001-5208-3432> ;
                                             <http://purl.org/dc/elements/1.1/date> "2018-09-14T20:19:56Z"^^xsd:dateTime ;
                                             rdfs:label "protocol creation role" .

[ rdf:type owl:Axiom ;
   owl:annotatedSource <http://purl.obolibrary.org/obo/CRO_0000053> ;
   owl:annotatedProperty <http://purl.obolibrary.org/obo/IAO_0000115> ;
   owl:annotatedTarget "A methodology role that involves creation of a detailed plan of a scientific or medical experiment, treatment, or procedure." ;
   <http://purl.obolibrary.org/obo/IAO_0000119> "https://www.merriam-webster.com/dictionary/protocol"
 ] .


###  http://purl.obolibrary.org/obo/CRO_0000054
<http://purl.obolibrary.org/obo/CRO_0000054> rdf:type owl:Class ;
                                             rdfs:subClassOf owl:Thing ;
                                             <http://purl.obolibrary.org/obo/IAO_0000115> "A methodology role that involves the development or creation of an established or prescribed methods to be followed routinely for the performance of designated operations or in designated situations." ;
                                             <http://purl.obolibrary.org/obo/IAO_0100001> <http://purl.obolibrary.org/obo/CRO_0000052> ;
                                             <http://purl.org/dc/elements/1.1/creator> <http://orcid.org/0000-0001-5208-3432> ;
                                             <http://purl.org/dc/elements/1.1/date> "2018-09-14T20:20:02Z"^^xsd:dateTime ;
                                             rdfs:label "obsolete standard operating procedure development role" ;
                                             owl:deprecated "true"^^xsd:boolean .

[ rdf:type owl:Axiom ;
   owl:annotatedSource <http://purl.obolibrary.org/obo/CRO_0000054> ;
   owl:annotatedProperty <http://purl.obolibrary.org/obo/IAO_0000115> ;
   owl:annotatedTarget "A methodology role that involves the development or creation of an established or prescribed methods to be followed routinely for the performance of designated operations or in designated situations." ;
   <http://purl.obolibrary.org/obo/IAO_0000119> "https://www.merriam-webster.com/dictionary/standard%20operating%20procedure"
 ] .


###  http://purl.obolibrary.org/obo/CRO_0000055
<http://purl.obolibrary.org/obo/CRO_0000055> rdf:type owl:Class ;
                                             rdfs:subClassOf <http://purl.org/credit/ontology#CREDIT_00000006> ;
                                             <http://purl.obolibrary.org/obo/IAO_0000115> "Detailed design of study components including data collection, analysis, and dissemination." ;
                                             <http://purl.org/dc/elements/1.1/creator> <http://orcid.org/0000-0001-5208-3432> ;
                                             <http://purl.org/dc/elements/1.1/date> "2018-09-14T20:20:06Z"^^xsd:dateTime ;
                                             rdfs:label "study design role" .


###  http://purl.obolibrary.org/obo/CRO_0000056
<http://purl.obolibrary.org/obo/CRO_0000056> rdf:type owl:Class ;
                                             rdfs:subClassOf <http://purl.org/credit/ontology#CREDIT_00000006> ;
                                             <http://purl.obolibrary.org/obo/IAO_0000115> "A methodology role that involves the creation or refinement of a manner or method by which an activity is performed." ;
                                             <http://purl.org/dc/elements/1.1/creator> <http://orcid.org/0000-0001-5208-3432> ;
                                             <http://purl.org/dc/elements/1.1/date> "2018-09-14T20:20:11Z"^^xsd:dateTime ;
                                             rdfs:label "technique development role" .

[ rdf:type owl:Axiom ;
   owl:annotatedSource <http://purl.obolibrary.org/obo/CRO_0000056> ;
   owl:annotatedProperty <http://purl.obolibrary.org/obo/IAO_0000115> ;
   owl:annotatedTarget "A methodology role that involves the creation or refinement of a manner or method by which an activity is performed." ;
   <http://purl.obolibrary.org/obo/IAO_0000119> "https://www.wikidata.org/wiki/Q2695280"
 ] .


###  http://purl.obolibrary.org/obo/CRO_0000057
<http://purl.obolibrary.org/obo/CRO_0000057> rdf:type owl:Class ;
                                             rdfs:subClassOf <http://purl.obolibrary.org/obo/CRO_0000026> ;
                                             <http://purl.obolibrary.org/obo/IAO_0000115> "A role charged with conceptualization, design, development and marketing of complex equipment." ;
                                             <http://purl.obolibrary.org/obo/IAO_0000118> "instrument development role" ;
                                             <http://purl.org/dc/elements/1.1/creator> <http://orcid.org/0000-0001-5208-3432> ;
                                             <http://purl.org/dc/elements/1.1/date> "2018-09-14T20:23:39Z"^^xsd:dateTime ;
                                             rdfs:label "device development role" .

[ rdf:type owl:Axiom ;
   owl:annotatedSource <http://purl.obolibrary.org/obo/CRO_0000057> ;
   owl:annotatedProperty <http://purl.obolibrary.org/obo/IAO_0000115> ;
   owl:annotatedTarget "A role charged with conceptualization, design, development and marketing of complex equipment." ;
   <http://purl.obolibrary.org/obo/IAO_0000119> "https://searchcio.techtarget.com/definition/product-development-or-new-product-development-NPD"
 ] .


###  http://purl.obolibrary.org/obo/CRO_0000058
<http://purl.obolibrary.org/obo/CRO_0000058> rdf:type owl:Class ;
                                             rdfs:subClassOf <http://purl.obolibrary.org/obo/CRO_0000026> ;
                                             <http://purl.obolibrary.org/obo/IAO_0000115> "A person that is responsible for operating equipment or instrumentation and/or that ensures equipment is well-maintained, properly configured, and safely functional." ;
                                             <http://purl.obolibrary.org/obo/IAO_0000118> "instrument technician role" ;
                                             <http://purl.org/dc/elements/1.1/creator> <http://orcid.org/0000-0001-5208-3432> ;
                                             <http://purl.org/dc/elements/1.1/date> "2018-09-14T20:23:44Z"^^xsd:dateTime ;
                                             rdfs:label "equipment technician role" .

[ rdf:type owl:Axiom ;
   owl:annotatedSource <http://purl.obolibrary.org/obo/CRO_0000058> ;
   owl:annotatedProperty <http://purl.obolibrary.org/obo/IAO_0000115> ;
   owl:annotatedTarget "A person that is responsible for operating equipment or instrumentation and/or that ensures equipment is well-maintained, properly configured, and safely functional." ;
   <http://purl.obolibrary.org/obo/IAO_0000119> "https://en.wikipedia.org/wiki/Biomedical_equipment_technician"
 ] .


###  http://purl.obolibrary.org/obo/CRO_0000059
<http://purl.obolibrary.org/obo/CRO_0000059> rdf:type owl:Class ;
                                             rdfs:subClassOf <http://purl.obolibrary.org/obo/CRO_0000106> ;
                                             <http://purl.obolibrary.org/obo/IAO_0000115> "Creation or refinement of a survey or questionnaire, a list of questions aimed at extracting specific data from a particular group of people." ;
                                             <http://purl.org/dc/elements/1.1/creator> <http://orcid.org/0000-0001-5208-3432> ;
                                             <http://purl.org/dc/elements/1.1/date> "2018-09-14T20:23:49Z"^^xsd:dateTime ;
                                             rdfs:label "survey and questionnaire development role" .

[ rdf:type owl:Axiom ;
   owl:annotatedSource <http://purl.obolibrary.org/obo/CRO_0000059> ;
   owl:annotatedProperty <http://purl.obolibrary.org/obo/IAO_0000115> ;
   owl:annotatedTarget "Creation or refinement of a survey or questionnaire, a list of questions aimed at extracting specific data from a particular group of people." ;
   <http://purl.obolibrary.org/obo/IAO_0000119> "https://www.wikidata.org/wiki/Q7257997"
 ] .


###  http://purl.obolibrary.org/obo/CRO_0000060
<http://purl.obolibrary.org/obo/CRO_0000060> rdf:type owl:Class ;
                                             rdfs:subClassOf <http://purl.obolibrary.org/obo/CRO_0000101> ,
                                                             <http://purl.org/credit/ontology#CREDIT_00000009> ;
                                             <http://purl.obolibrary.org/obo/IAO_0000115> "Examination of software code to identify build-breaking changes prior to acceptance into a codebase." ;
                                             <http://purl.obolibrary.org/obo/IAO_0000118> "software code review role" ;
                                             <http://purl.org/dc/elements/1.1/creator> <http://orcid.org/0000-0001-5208-3432> ;
                                             <http://purl.org/dc/elements/1.1/date> "2018-09-14T20:25:30Z"^^xsd:dateTime ;
                                             rdfs:label "code review role" .


###  http://purl.obolibrary.org/obo/CRO_0000061
<http://purl.obolibrary.org/obo/CRO_0000061> rdf:type owl:Class ;
                                             rdfs:subClassOf owl:Thing ;
                                             <http://purl.obolibrary.org/obo/IAO_0000115> "Algorithm development and implementation of software in a computer programming language." ;
                                             <http://purl.obolibrary.org/obo/IAO_0100001> <http://purl.obolibrary.org/obo/CRO_0000064> ;
                                             <http://purl.org/dc/elements/1.1/creator> <http://orcid.org/0000-0001-5208-3432> ;
                                             <http://purl.org/dc/elements/1.1/date> "2018-09-14T20:25:35Z"^^xsd:dateTime ;
                                             rdfs:label "obsolete computer programming role" ;
                                             owl:deprecated "true"^^xsd:boolean .


###  http://purl.obolibrary.org/obo/CRO_0000062
<http://purl.obolibrary.org/obo/CRO_0000062> rdf:type owl:Class ;
                                             rdfs:subClassOf <http://purl.org/credit/ontology#CREDIT_00000009> ;
                                             <http://purl.obolibrary.org/obo/IAO_0000115> "Creation of high-level structures of a software system." ;
                                             <http://purl.org/dc/elements/1.1/creator> <http://orcid.org/0000-0001-5208-3432> ;
                                             <http://purl.org/dc/elements/1.1/date> "2018-09-14T20:25:40Z"^^xsd:dateTime ;
                                             rdfs:label "software architecture role" .


###  http://purl.obolibrary.org/obo/CRO_0000063
<http://purl.obolibrary.org/obo/CRO_0000063> rdf:type owl:Class ;
                                             rdfs:subClassOf <http://purl.org/credit/ontology#CREDIT_00000009> ;
                                             <http://purl.obolibrary.org/obo/IAO_0000115> "Creation of low-level software component and algorithm design." ;
                                             <http://purl.org/dc/elements/1.1/creator> <http://orcid.org/0000-0001-5208-3432> ;
                                             <http://purl.org/dc/elements/1.1/date> "2018-09-14T20:25:45Z"^^xsd:dateTime ;
                                             rdfs:label "software design role" .

[ rdf:type owl:Axiom ;
   owl:annotatedSource <http://purl.obolibrary.org/obo/CRO_0000063> ;
   owl:annotatedProperty <http://purl.obolibrary.org/obo/IAO_0000115> ;
   owl:annotatedTarget "Creation of low-level software component and algorithm design." ;
   <http://purl.obolibrary.org/obo/IAO_0000119> "https://en.wikipedia.org/wiki/Low-level_design"
 ] .


###  http://purl.obolibrary.org/obo/CRO_0000064
<http://purl.obolibrary.org/obo/CRO_0000064> rdf:type owl:Class ;
                                             rdfs:subClassOf <http://purl.org/credit/ontology#CREDIT_00000009> ;
                                             <http://purl.obolibrary.org/obo/IAO_0000115> "Systematic application of scientific and technological knowledge, methods, and experience to the design, implementation, testing, and documentation of software." ;
                                             <http://purl.obolibrary.org/obo/IAO_0000118> "computer programming role" ;
                                             <http://purl.org/dc/elements/1.1/creator> <http://orcid.org/0000-0001-5208-3432> ;
                                             <http://purl.org/dc/elements/1.1/date> "2018-09-14T20:25:49Z"^^xsd:dateTime ;
                                             rdfs:label "software engineering role" .


###  http://purl.obolibrary.org/obo/CRO_0000065
<http://purl.obolibrary.org/obo/CRO_0000065> rdf:type owl:Class ;
                                             rdfs:subClassOf <http://purl.obolibrary.org/obo/CRO_0000078> ;
                                             <http://purl.obolibrary.org/obo/IAO_0000115> "Planning, management, and monitoring of projects." ;
                                             <http://purl.org/dc/elements/1.1/creator> <http://orcid.org/0000-0001-5208-3432> ;
                                             <http://purl.org/dc/elements/1.1/date> "2018-09-14T20:25:55Z"^^xsd:dateTime ;
                                             rdfs:label "project management role" .


###  http://purl.obolibrary.org/obo/CRO_0000067
<http://purl.obolibrary.org/obo/CRO_0000067> rdf:type owl:Class ;
                                             rdfs:subClassOf <http://purl.obolibrary.org/obo/CRO_0000023> ;
                                             <http://purl.obolibrary.org/obo/IAO_0000115> "A professional who assesses, collects, organizes, preserves, maintains control over, and provides access to information determined to have long-term value." ;
                                             <http://purl.org/dc/elements/1.1/creator> <http://orcid.org/0000-0001-5208-3432> ;
                                             <http://purl.org/dc/elements/1.1/date> "2018-09-15T16:25:54Z"^^xsd:dateTime ;
                                             rdfs:label "archivist role" .

[ rdf:type owl:Axiom ;
   owl:annotatedSource <http://purl.obolibrary.org/obo/CRO_0000067> ;
   owl:annotatedProperty <http://purl.obolibrary.org/obo/IAO_0000115> ;
   owl:annotatedTarget "A professional who assesses, collects, organizes, preserves, maintains control over, and provides access to information determined to have long-term value." ;
   <http://purl.obolibrary.org/obo/IAO_0000119> "https://www.wikidata.org/wiki/Q635734"
 ] .


###  http://purl.obolibrary.org/obo/CRO_0000068
<http://purl.obolibrary.org/obo/CRO_0000068> rdf:type owl:Class ;
                                             rdfs:subClassOf <http://purl.obolibrary.org/obo/CRO_0000023> ;
                                             <http://purl.obolibrary.org/obo/IAO_0000115> "A person responsible for the preservation of artistic and cultural artifacts." ;
                                             <http://purl.org/dc/elements/1.1/creator> <http://orcid.org/0000-0001-5208-3432> ;
                                             <http://purl.org/dc/elements/1.1/date> "2018-09-15T16:26:00Z"^^xsd:dateTime ;
                                             rdfs:label "conservator role" .

[ rdf:type owl:Axiom ;
   owl:annotatedSource <http://purl.obolibrary.org/obo/CRO_0000068> ;
   owl:annotatedProperty <http://purl.obolibrary.org/obo/IAO_0000115> ;
   owl:annotatedTarget "A person responsible for the preservation of artistic and cultural artifacts." ;
   <http://purl.obolibrary.org/obo/IAO_0000119> "https://www.wikidata.org/wiki/Q446966"
 ] .


###  http://purl.obolibrary.org/obo/CRO_0000069
<http://purl.obolibrary.org/obo/CRO_0000069> rdf:type owl:Class ;
                                             rdfs:subClassOf <http://purl.obolibrary.org/obo/CRO_0000023> ;
                                             <http://purl.obolibrary.org/obo/IAO_0000115> "A role that includes the formal endeavor to ensure that digital information of continuing value remains accessible, trustworthy, and usable." ;
                                             <http://purl.org/dc/elements/1.1/creator> <http://orcid.org/0000-0001-5208-3432> ;
                                             <http://purl.org/dc/elements/1.1/date> "2018-09-15T16:26:05Z"^^xsd:dateTime ;
                                             rdfs:label "digital preservation role" .

[ rdf:type owl:Axiom ;
   owl:annotatedSource <http://purl.obolibrary.org/obo/CRO_0000069> ;
   owl:annotatedProperty <http://purl.obolibrary.org/obo/IAO_0000115> ;
   owl:annotatedTarget "A role that includes the formal endeavor to ensure that digital information of continuing value remains accessible, trustworthy, and usable." ;
   <http://purl.obolibrary.org/obo/IAO_0000119> "https://www.wikidata.org/wiki/Q632897"
 ] .


###  http://purl.obolibrary.org/obo/CRO_0000070
<http://purl.obolibrary.org/obo/CRO_0000070> rdf:type owl:Class ;
                                             rdfs:subClassOf owl:Thing ;
                                             <http://purl.org/dc/elements/1.1/creator> <http://orcid.org/0000-0001-5208-3432> ;
                                             <http://purl.org/dc/elements/1.1/date> "2018-09-15T16:29:29Z"^^xsd:dateTime ;
                                             rdfs:label "relationship" .


###  http://purl.obolibrary.org/obo/CRO_0000071
<http://purl.obolibrary.org/obo/CRO_0000071> rdf:type owl:Class ;
                                             rdfs:subClassOf <http://purl.obolibrary.org/obo/CRO_0000070> ;
                                             <http://purl.org/dc/elements/1.1/creator> <http://orcid.org/0000-0001-5208-3432> ;
                                             <http://purl.org/dc/elements/1.1/date> "2018-09-15T16:29:43Z"^^xsd:dateTime ;
                                             rdfs:label "contributorship" .


###  http://purl.obolibrary.org/obo/CRO_0000072
<http://purl.obolibrary.org/obo/CRO_0000072> rdf:type owl:Class ;
                                             rdfs:subClassOf <http://purl.obolibrary.org/obo/CRO_0000015> ;
                                             <http://purl.obolibrary.org/obo/IAO_0000115> "Aggregation, integration, manipulation of data." ;
                                             <http://purl.obolibrary.org/obo/IAO_0000118> "data manipulation role" ;
                                             <http://purl.org/dc/elements/1.1/creator> <http://orcid.org/0000-0001-5208-3432> ;
                                             <http://purl.org/dc/elements/1.1/date> "2018-10-01T20:32:37Z"^^xsd:dateTime ;
                                             rdfs:label "data transformation role" .


###  http://purl.obolibrary.org/obo/CRO_0000073
<http://purl.obolibrary.org/obo/CRO_0000073> rdf:type owl:Class ;
                                             rdfs:subClassOf <http://purl.obolibrary.org/obo/CRO_0000000> ;
                                             <http://purl.obolibrary.org/obo/IAO_0000115> "The process of creating standards, which aare an established norm or requirement in regard to technical systems. It is usually a formal document that establishes uniform engineering or technical criteria, methods, processes, and practices." ;
                                             <http://purl.obolibrary.org/obo/IAO_0000118> "standard development role" ;
                                             <http://purl.org/dc/elements/1.1/creator> <http://orcid.org/0000-0001-5208-3432> ;
                                             <http://purl.org/dc/elements/1.1/date> "2018-10-01T20:33:58Z"^^xsd:dateTime ;
                                             rdfs:label "standards development role" .

[ rdf:type owl:Axiom ;
   owl:annotatedSource <http://purl.obolibrary.org/obo/CRO_0000073> ;
   owl:annotatedProperty <http://purl.obolibrary.org/obo/IAO_0000115> ;
   owl:annotatedTarget "The process of creating standards, which aare an established norm or requirement in regard to technical systems. It is usually a formal document that establishes uniform engineering or technical criteria, methods, processes, and practices." ;
   <http://purl.obolibrary.org/obo/IAO_0000119> "https://en.wikipedia.org/wiki/Technical_standard"
 ] .


###  http://purl.obolibrary.org/obo/CRO_0000074
<http://purl.obolibrary.org/obo/CRO_0000074> rdf:type owl:Class ;
                                             rdfs:subClassOf <http://purl.obolibrary.org/obo/CRO_0000015> ;
                                             <http://purl.obolibrary.org/obo/IAO_0000115> "Verification, whether as a part of the activity or separate, of the overall replication/reproducibility of results/experiments and other research outputs." ;
                                             <http://purl.org/dc/elements/1.1/creator> <http://orcid.org/0000-0001-5208-3432> ;
                                             <http://purl.org/dc/elements/1.1/date> "2018-10-01T20:35:43Z"^^xsd:dateTime ;
                                             rdfs:label "data validation role" .


###  http://purl.obolibrary.org/obo/CRO_0000075
<http://purl.obolibrary.org/obo/CRO_0000075> rdf:type owl:Class ;
                                             rdfs:subClassOf owl:Thing ;
                                             <http://purl.obolibrary.org/obo/IAO_0000118> "formal training role" ;
                                             <http://purl.obolibrary.org/obo/IAO_0100001> <http://purl.obolibrary.org/obo/CRO_0000047> ;
                                             <http://purl.org/dc/elements/1.1/creator> <http://orcid.org/0000-0001-5208-3432> ;
                                             <http://purl.org/dc/elements/1.1/date> "2018-10-01T20:42:52Z"^^xsd:dateTime ;
                                             rdfs:label "educational training role" ;
                                             owl:deprecated "true"^^xsd:boolean .


###  http://purl.obolibrary.org/obo/CRO_0000076
<http://purl.obolibrary.org/obo/CRO_0000076> rdf:type owl:Class ;
                                             rdfs:subClassOf owl:Thing ;
                                             <http://purl.obolibrary.org/obo/IAO_0000115> "A role that includes the design and implementation of the physical components of a computer system." ;
                                             <http://purl.obolibrary.org/obo/IAO_0000118> "information technology hardware systems design and implementation role" ;
                                             <http://purl.org/dc/elements/1.1/creator> <http://orcid.org/0000-0001-5208-3432> ;
                                             <http://purl.org/dc/elements/1.1/date> "2018-10-01T20:43:37Z"^^xsd:dateTime ;
                                             rdfs:label "obsolete IT hardware systems design and implementation role" ;
                                             owl:deprecated "true"^^xsd:boolean .

[ rdf:type owl:Axiom ;
   owl:annotatedSource <http://purl.obolibrary.org/obo/CRO_0000076> ;
   owl:annotatedProperty <http://purl.obolibrary.org/obo/IAO_0000115> ;
   owl:annotatedTarget "A role that includes the design and implementation of the physical components of a computer system." ;
   <http://purl.obolibrary.org/obo/IAO_0000119> "https://www.wikidata.org/wiki/Q3966"
 ] .


###  http://purl.obolibrary.org/obo/CRO_0000077
<http://purl.obolibrary.org/obo/CRO_0000077> rdf:type owl:Class ;
                                             rdfs:subClassOf owl:Thing ;
                                             <http://purl.obolibrary.org/obo/IAO_0100001> <http://purl.obolibrary.org/obo/CRO_0000051> ;
                                             <http://purl.org/dc/elements/1.1/creator> <http://orcid.org/0000-0001-5208-3432> ;
                                             <http://purl.org/dc/elements/1.1/date> "2018-10-01T20:44:21Z"^^xsd:dateTime ;
                                             rdfs:label "systems administration role" ;
                                             owl:deprecated "true"^^xsd:boolean .


###  http://purl.obolibrary.org/obo/CRO_0000078
<http://purl.obolibrary.org/obo/CRO_0000078> rdf:type owl:Class ;
                                             rdfs:subClassOf <http://purl.obolibrary.org/obo/CRO_0000000> ;
                                             <http://purl.obolibrary.org/obo/IAO_0000115> "Contribution to the basic, underlying framework or features of a system or organization." ;
                                             <http://purl.org/dc/elements/1.1/creator> <http://orcid.org/0000-0001-5208-3432> ;
                                             <http://purl.org/dc/elements/1.1/date> "2018-10-01T20:48:11Z"^^xsd:dateTime ;
                                             rdfs:label "infrastructure role" .

[ rdf:type owl:Axiom ;
   owl:annotatedSource <http://purl.obolibrary.org/obo/CRO_0000078> ;
   owl:annotatedProperty <http://purl.obolibrary.org/obo/IAO_0000115> ;
   owl:annotatedTarget "Contribution to the basic, underlying framework or features of a system or organization." ;
   <http://purl.obolibrary.org/obo/IAO_0000119> "https://www.dictionary.com/browse/infrastructure"
 ] .


###  http://purl.obolibrary.org/obo/CRO_0000079
<http://purl.obolibrary.org/obo/CRO_0000079> rdf:type owl:Class ;
                                             rdfs:subClassOf <http://purl.obolibrary.org/obo/CRO_0000078> ;
                                             <http://purl.obolibrary.org/obo/IAO_0000115> "Evaluation is a systematic method for collecting, analyzing, and using information to answer questions about projects, policies and programs, particularly about their effectiveness and efficiency." ;
                                             <http://purl.org/dc/elements/1.1/creator> <http://orcid.org/0000-0001-5208-3432> ;
                                             <http://purl.org/dc/elements/1.1/date> "2018-10-01T20:48:24Z"^^xsd:dateTime ;
                                             rdfs:label "project, policy or program evaluation role" .

[ rdf:type owl:Axiom ;
   owl:annotatedSource <http://purl.obolibrary.org/obo/CRO_0000079> ;
   owl:annotatedProperty <http://purl.obolibrary.org/obo/IAO_0000115> ;
   owl:annotatedTarget "Evaluation is a systematic method for collecting, analyzing, and using information to answer questions about projects, policies and programs, particularly about their effectiveness and efficiency." ;
   <http://purl.obolibrary.org/obo/IAO_0000119> "https://en.wikipedia.org/wiki/Program_evaluation"
 ] .


###  http://purl.obolibrary.org/obo/CRO_0000080
<http://purl.obolibrary.org/obo/CRO_0000080> rdf:type owl:Class ;
                                             rdfs:subClassOf owl:Thing ;
                                             <http://purl.obolibrary.org/obo/IAO_0000115> "An infrastructure role that is accountable for management and coordination of a program, to help achieve the program goals." ;
                                             <http://purl.obolibrary.org/obo/IAO_0100001> <http://purl.org/credit/ontology#CREDIT_00000007> ;
                                             <http://purl.org/dc/elements/1.1/creator> <http://orcid.org/0000-0001-5208-3432> ;
                                             <http://purl.org/dc/elements/1.1/date> "2018-10-01T20:48:37Z"^^xsd:dateTime ;
                                             rdfs:label "obsolete program administration role" ;
                                             owl:deprecated "true"^^xsd:boolean .


###  http://purl.obolibrary.org/obo/CRO_0000081
<http://purl.obolibrary.org/obo/CRO_0000081> rdf:type owl:Class ;
                                             rdfs:subClassOf <http://purl.obolibrary.org/obo/CRO_0000078> ;
                                             <http://purl.obolibrary.org/obo/IAO_0000115> "The organization of the different elements needed to implement a study." ;
                                             <http://purl.org/dc/elements/1.1/creator> <http://orcid.org/0000-0001-5208-3432> ;
                                             <http://purl.org/dc/elements/1.1/date> "2018-10-01T20:49:10Z"^^xsd:dateTime ;
                                             rdfs:label "coordination role" .

[ rdf:type owl:Axiom ;
   owl:annotatedSource <http://purl.obolibrary.org/obo/CRO_0000081> ;
   owl:annotatedProperty <http://purl.obolibrary.org/obo/IAO_0000115> ;
   owl:annotatedTarget "The organization of the different elements needed to implement a study." ;
   <http://purl.obolibrary.org/obo/IAO_0000119> "https://learn.nursing.jhu.edu/face-to-face/courses/research-coordinator/index.html"
 ] .


###  http://purl.obolibrary.org/obo/CRO_0000082
<http://purl.obolibrary.org/obo/CRO_0000082> rdf:type owl:Class ;
                                             rdfs:subClassOf owl:Thing ;
                                             <http://purl.obolibrary.org/obo/IAO_0000115> "Oversight and leadership responsibility for the research activity planning and execution, including mentorship external to the core team." ;
                                             <http://purl.obolibrary.org/obo/IAO_0100001> <http://purl.org/credit/ontology#CREDIT_00000010> ;
                                             <http://purl.org/dc/elements/1.1/creator> <http://orcid.org/0000-0001-5208-3432> ;
                                             <http://purl.org/dc/elements/1.1/date> "2018-10-01T20:49:54Z"^^xsd:dateTime ;
                                             rdfs:label "supervisory role" ;
                                             owl:deprecated "true"^^xsd:boolean .


###  http://purl.obolibrary.org/obo/CRO_0000083
<http://purl.obolibrary.org/obo/CRO_0000083> rdf:type owl:Class ;
                                             rdfs:subClassOf <http://purl.obolibrary.org/obo/CRO_0000007> ;
                                             <http://purl.obolibrary.org/obo/IAO_0000115> "A communication role which involves the dynamic relational process that facilitates communication, interaction, involvement, and exchange between an organization and a community for a range of social and organizational outcomes." ;
                                             <http://purl.org/dc/elements/1.1/creator> <http://orcid.org/0000-0001-5208-3432> ;
                                             <http://purl.org/dc/elements/1.1/date> "2018-10-01T20:55:22Z"^^xsd:dateTime ;
                                             rdfs:label "community engagement role" .

[ rdf:type owl:Axiom ;
   owl:annotatedSource <http://purl.obolibrary.org/obo/CRO_0000083> ;
   owl:annotatedProperty <http://purl.obolibrary.org/obo/IAO_0000115> ;
   owl:annotatedTarget "A communication role which involves the dynamic relational process that facilitates communication, interaction, involvement, and exchange between an organization and a community for a range of social and organizational outcomes." ;
   <http://purl.obolibrary.org/obo/IAO_0000119> "Johnston, K. A. (2018). Toward a theory of social engagement. In K. A. Johnston & M. Taylor (Eds.), The Handbook of Communication Engagement (pp. 19-32). Hoboken, NJ: Wiley."
 ] .


###  http://purl.obolibrary.org/obo/CRO_0000084
<http://purl.obolibrary.org/obo/CRO_0000084> rdf:type owl:Class ;
                                             rdfs:subClassOf <http://purl.obolibrary.org/obo/CRO_0000007> ;
                                             <http://purl.obolibrary.org/obo/IAO_0000115> "A communication role that involves development or production of materials, such as brochures, websites, flyers, presentations, etc., for the purposes of promotion of a entity, like a project, group or organization." ;
                                             <http://purl.org/dc/elements/1.1/creator> <http://orcid.org/0000-0001-5208-3432> ;
                                             <http://purl.org/dc/elements/1.1/date> "2018-10-01T20:56:18Z"^^xsd:dateTime ;
                                             rdfs:label "outreach materials development role" .


###  http://purl.obolibrary.org/obo/CRO_0000085
<http://purl.obolibrary.org/obo/CRO_0000085> rdf:type owl:Class ;
                                             rdfs:subClassOf owl:Thing ;
                                             <http://purl.obolibrary.org/obo/IAO_0000115> "Role that involves identifying eligible participants, explaining the study to potential participants, recruiting an adequate sample based on study goals and design, obtaining informed consent/maintaining ethical standards, and retaining participants until study completion." ;
                                             <http://purl.org/dc/elements/1.1/creator> <http://orcid.org/0000-0001-5208-3432> ;
                                             <http://purl.org/dc/elements/1.1/date> "2018-10-01T20:57:17Z"^^xsd:dateTime ;
                                             rdfs:label "obsolete participant recruitment role" ;
                                             owl:deprecated "true"^^xsd:boolean .

[ rdf:type owl:Axiom ;
   owl:annotatedSource <http://purl.obolibrary.org/obo/CRO_0000085> ;
   owl:annotatedProperty <http://purl.obolibrary.org/obo/IAO_0000115> ;
   owl:annotatedTarget "Role that involves identifying eligible participants, explaining the study to potential participants, recruiting an adequate sample based on study goals and design, obtaining informed consent/maintaining ethical standards, and retaining participants until study completion." ;
   <http://purl.obolibrary.org/obo/IAO_0000119> "https://healthit.ahrq.gov/ahrq-funded-projects/emerging-lessons/participant-recruitment-research"
 ] .


###  http://purl.obolibrary.org/obo/CRO_0000086
<http://purl.obolibrary.org/obo/CRO_0000086> rdf:type owl:Class ;
                                             rdfs:subClassOf owl:Thing ;
                                             <http://purl.obolibrary.org/obo/IAO_0000118> "Ideas; formulation or evolution of overarching research goals and aims." ;
                                             <http://purl.obolibrary.org/obo/IAO_0100001> <http://purl.org/credit/ontology#CREDIT_00000001> ;
                                             <http://purl.org/dc/elements/1.1/creator> <http://orcid.org/0000-0001-5208-3432> ;
                                             <http://purl.org/dc/elements/1.1/date> "2018-10-01T20:57:53Z"^^xsd:dateTime ;
                                             rdfs:label "research conceptualization role" ;
                                             owl:deprecated "true"^^xsd:boolean .


###  http://purl.obolibrary.org/obo/CRO_0000087
<http://purl.obolibrary.org/obo/CRO_0000087> rdf:type owl:Class ;
                                             rdfs:subClassOf <http://purl.org/credit/ontology#CREDIT_00000005> ;
                                             <http://purl.obolibrary.org/obo/IAO_0000115> "One who is proficient in the relevant skill and technique, with a relatively practical understanding of the theoretical principles." ;
                                             <http://purl.org/dc/elements/1.1/creator> <http://orcid.org/0000-0001-5208-3432> ;
                                             <http://purl.org/dc/elements/1.1/date> "2018-10-01T20:58:59Z"^^xsd:dateTime ;
                                             rdfs:label "technician role" .

[ rdf:type owl:Axiom ;
   owl:annotatedSource <http://purl.obolibrary.org/obo/CRO_0000087> ;
   owl:annotatedProperty <http://purl.obolibrary.org/obo/IAO_0000115> ;
   owl:annotatedTarget "One who is proficient in the relevant skill and technique, with a relatively practical understanding of the theoretical principles." ;
   <http://purl.obolibrary.org/obo/IAO_0000119> "https://en.wikipedia.org/wiki/Technician"
 ] .


###  http://purl.obolibrary.org/obo/CRO_0000088
<http://purl.obolibrary.org/obo/CRO_0000088> rdf:type owl:Class ;
                                             rdfs:subClassOf owl:Thing ;
                                             <http://purl.obolibrary.org/obo/IAO_0000115> "Creation and/or presentation of the published work, specifically writing the initial draft (including substantive translation)." ;
                                             <http://purl.obolibrary.org/obo/IAO_0100001> <http://purl.org/credit/ontology#CREDIT_00000013> ;
                                             <http://purl.org/dc/elements/1.1/creator> <http://orcid.org/0000-0001-5208-3432> ;
                                             <http://purl.org/dc/elements/1.1/date> "2018-10-01T21:03:36Z"^^xsd:dateTime ;
                                             rdfs:label "original draft preparation role" ;
                                             owl:deprecated "true"^^xsd:boolean .


###  http://purl.obolibrary.org/obo/CRO_0000089
<http://purl.obolibrary.org/obo/CRO_0000089> rdf:type owl:Class ;
                                             rdfs:subClassOf <http://purl.obolibrary.org/obo/CRO_0000001> ;
                                             <http://purl.obolibrary.org/obo/IAO_0000115> "A role in which one provides a summary of a research output, such as a journal article, that is understandable by a lay person or non-expert audience." ;
                                             <http://purl.obolibrary.org/obo/IAO_0000118> "lay synthesis of research output role" ;
                                             <http://purl.org/dc/elements/1.1/creator> <http://orcid.org/0000-0001-5208-3432> ;
                                             <http://purl.org/dc/elements/1.1/date> "2018-10-01T21:04:14Z"^^xsd:dateTime ;
                                             rdfs:label "lay summary role" .


###  http://purl.obolibrary.org/obo/CRO_0000090
<http://purl.obolibrary.org/obo/CRO_0000090> rdf:type owl:Class ;
                                             rdfs:subClassOf owl:Thing ;
                                             <http://purl.obolibrary.org/obo/IAO_0000115> "A method or steps that maintain, update content, clean up, or repair a website." ;
                                             <http://purl.obolibrary.org/obo/IAO_0100001> <http://purl.obolibrary.org/obo/CRO_0000008> ;
                                             <http://purl.org/dc/elements/1.1/creator> <http://orcid.org/0000-0001-5208-3432> ;
                                             <http://purl.org/dc/elements/1.1/date> "2018-10-01T21:13:13Z"^^xsd:dateTime ;
                                             rdfs:label "obsolete website maintenance role" ;
                                             owl:deprecated "true"^^xsd:boolean .

[ rdf:type owl:Axiom ;
   owl:annotatedSource <http://purl.obolibrary.org/obo/CRO_0000090> ;
   owl:annotatedProperty <http://purl.obolibrary.org/obo/IAO_0000115> ;
   owl:annotatedTarget "A method or steps that maintain, update content, clean up, or repair a website." ;
   <http://purl.obolibrary.org/obo/IAO_0000119> "https://www.wikidata.org/wiki/Q17634596"
 ] .


###  http://purl.obolibrary.org/obo/CRO_0000091
<http://purl.obolibrary.org/obo/CRO_0000091> rdf:type owl:Class ;
                                             rdfs:subClassOf <http://purl.obolibrary.org/obo/CRO_0000011> ;
                                             <http://purl.obolibrary.org/obo/IAO_0000115> "A documentation role that involves preparation of instruction manuals, journal articles, and other supporting documents to communicate complex and technical information more easily." ;
                                             <http://www.geneontology.org/formats/oboInOwl#created_by> <http://orcid.org/0000-0001-5208-3432> ;
                                             rdfs:label "technical writing role" .

[ rdf:type owl:Axiom ;
   owl:annotatedSource <http://purl.obolibrary.org/obo/CRO_0000091> ;
   owl:annotatedProperty <http://purl.obolibrary.org/obo/IAO_0000115> ;
   owl:annotatedTarget "A documentation role that involves preparation of instruction manuals, journal articles, and other supporting documents to communicate complex and technical information more easily." ;
   <http://purl.obolibrary.org/obo/IAO_0000119> "https://www.truity.com/career-profile/technical-writer"
 ] .


###  http://purl.obolibrary.org/obo/CRO_0000092
<http://purl.obolibrary.org/obo/CRO_0000092> rdf:type owl:Class ;
                                             rdfs:subClassOf <http://purl.org/credit/ontology#CREDIT_00000009> ;
                                             <http://purl.obolibrary.org/obo/IAO_0000115> "The tasks that go into determining the needs or conditions to meet for a new or altered software product or project, taking account of the possibly conflicting requirements of the various stakeholders, analyzing, documenting, validating and managing software or system requirements." ;
                                             <http://www.geneontology.org/formats/oboInOwl#created_by> <http://orcid.org/0000-0001-5208-3432> ;
                                             rdfs:label "requirements analysis role" .

[ rdf:type owl:Axiom ;
   owl:annotatedSource <http://purl.obolibrary.org/obo/CRO_0000092> ;
   owl:annotatedProperty <http://purl.obolibrary.org/obo/IAO_0000115> ;
   owl:annotatedTarget "The tasks that go into determining the needs or conditions to meet for a new or altered software product or project, taking account of the possibly conflicting requirements of the various stakeholders, analyzing, documenting, validating and managing software or system requirements." ;
   <http://purl.obolibrary.org/obo/IAO_0000119> "Kotonya, G. and Sommerville, I. 1998. Requirements Engineering: Processes and Techniques Chichester, UK: John Wiley and Sons."
 ] .


###  http://purl.obolibrary.org/obo/CRO_0000093
<http://purl.obolibrary.org/obo/CRO_0000093> rdf:type owl:Class ;
                                             rdfs:subClassOf <http://purl.obolibrary.org/obo/CRO_0000028> ;
                                             <http://purl.obolibrary.org/obo/IAO_0000115> "Obtaining a material entity for potential use as an input during an investigation." ;
                                             <http://purl.obolibrary.org/obo/IAO_0000234> "https://orcid.org/0000-0002-2908-3327" ;
                                             <http://www.geneontology.org/formats/oboInOwl#created_by> <http://orcid.org/0000-0001-5208-3432> ;
                                             rdfs:label "specimen collection role" .


###  http://purl.obolibrary.org/obo/CRO_0000094
<http://purl.obolibrary.org/obo/CRO_0000094> rdf:type owl:Class ;
                                             rdfs:subClassOf <http://purl.obolibrary.org/obo/CRO_0000093> ;
                                             <http://purl.obolibrary.org/obo/IAO_0000115> "In botany, this is the collector listed first for a particular specimen. Each specimen has one primary collector. The primary collector assigns a number to that specimen from his/her own number series." ;
                                             <http://purl.obolibrary.org/obo/IAO_0000234> "http://orcid.org/0000-0002-2908-3327" ;
                                             <http://www.geneontology.org/formats/oboInOwl#created_by> <http://orcid.org/0000-0001-5208-3432> ;
                                             rdfs:label "primary collector role" .


###  http://purl.obolibrary.org/obo/CRO_0000095
<http://purl.obolibrary.org/obo/CRO_0000095> rdf:type owl:Class ;
                                             rdfs:subClassOf <http://purl.obolibrary.org/obo/CRO_0000101> ;
                                             <http://purl.obolibrary.org/obo/IAO_0000115> "Evaluation of grant applications by others working in the same field." ;
                                             <http://purl.obolibrary.org/obo/IAO_0000234> "https://orcid.org/0000-0001-9114-8737" ;
                                             <http://www.geneontology.org/formats/oboInOwl#created_by> <http://orcid.org/0000-0001-5208-3432> ;
                                             rdfs:label "grant peer review role" .


###  http://purl.obolibrary.org/obo/CRO_0000096
<http://purl.obolibrary.org/obo/CRO_0000096> rdf:type owl:Class ;
                                             rdfs:subClassOf <http://purl.obolibrary.org/obo/CRO_0000028> ;
                                             <http://purl.obolibrary.org/obo/IAO_0000115> "Selecting, ordering, and receiving materials or physical objects for research, scholarly, library or archival collections." ;
                                             <http://purl.obolibrary.org/obo/IAO_0000234> "https://orcid.org/0000-0002-2908-3327" ;
                                             <http://www.geneontology.org/formats/oboInOwl#created_by> <http://orcid.org/0000-0001-5208-3432> ;
                                             rdfs:label "acquisition role" .


###  http://purl.obolibrary.org/obo/CRO_0000097
<http://purl.obolibrary.org/obo/CRO_0000097> rdf:type owl:Class ;
                                             rdfs:subClassOf <http://purl.obolibrary.org/obo/CRO_0000000> ;
                                             <http://purl.obolibrary.org/obo/IAO_0000115> "The person or organization that provides money for a particular purpose, such as a grant to perform research." ;
                                             <http://purl.obolibrary.org/obo/IAO_0000118> "funder role" ;
                                             <http://www.geneontology.org/formats/oboInOwl#created_by> <http://orcid.org/0000-0001-5208-3432> ;
                                             rdfs:label "funding source role" .

[ rdf:type owl:Axiom ;
   owl:annotatedSource <http://purl.obolibrary.org/obo/CRO_0000097> ;
   owl:annotatedProperty <http://purl.obolibrary.org/obo/IAO_0000115> ;
   owl:annotatedTarget "The person or organization that provides money for a particular purpose, such as a grant to perform research." ;
   <http://purl.obolibrary.org/obo/IAO_0000119> "https://www.lexico.com/en/definition/funder"
 ] .


###  http://purl.obolibrary.org/obo/CRO_0000098
<http://purl.obolibrary.org/obo/CRO_0000098> rdf:type owl:Class ;
                                             rdfs:subClassOf <http://purl.obolibrary.org/obo/CRO_0000000> ;
                                             <http://purl.obolibrary.org/obo/IAO_0000115> "The person or organization that is responsible for a new or novel discovery, i.e., the process of finding information, a place, or an object, especially for the first time, or the thing that is found. For example, a researcher discovering a new gene mutation that contributes to a disease." ;
                                             <http://www.geneontology.org/formats/oboInOwl#created_by> <http://orcid.org/0000-0001-5208-3432> ;
                                             rdfs:label "discovery role" .

[ rdf:type owl:Axiom ;
   owl:annotatedSource <http://purl.obolibrary.org/obo/CRO_0000098> ;
   owl:annotatedProperty <http://purl.obolibrary.org/obo/IAO_0000115> ;
   owl:annotatedTarget "The person or organization that is responsible for a new or novel discovery, i.e., the process of finding information, a place, or an object, especially for the first time, or the thing that is found. For example, a researcher discovering a new gene mutation that contributes to a disease." ;
   <http://purl.obolibrary.org/obo/IAO_0000119> "https://dictionary.cambridge.org/us/dictionary/english/discovery"
 ] .


###  http://purl.obolibrary.org/obo/CRO_0000099
<http://purl.obolibrary.org/obo/CRO_0000099> rdf:type owl:Class ;
                                             rdfs:subClassOf <http://purl.obolibrary.org/obo/CRO_0000000> ;
                                             <http://purl.obolibrary.org/obo/IAO_0000115> "A person or organization who helps guide a patient through the healthcare system. This includes help going through the screening, diagnosis, treatment (including clinical trials), and follow-up of a medical condition, such as cancer." ;
                                             <http://www.geneontology.org/formats/oboInOwl#created_by> <http://orcid.org/0000-0001-5208-3432> ;
                                             rdfs:label "patient advocate role" .

[ rdf:type owl:Axiom ;
   owl:annotatedSource <http://purl.obolibrary.org/obo/CRO_0000099> ;
   owl:annotatedProperty <http://purl.obolibrary.org/obo/IAO_0000115> ;
   owl:annotatedTarget "A person or organization who helps guide a patient through the healthcare system. This includes help going through the screening, diagnosis, treatment (including clinical trials), and follow-up of a medical condition, such as cancer." ;
   <http://purl.obolibrary.org/obo/IAO_0000119> "https://www.cancer.gov/publications/dictionaries/cancer-terms/def/patient-advocate"
 ] .


###  http://purl.obolibrary.org/obo/CRO_0000100
<http://purl.obolibrary.org/obo/CRO_0000100> rdf:type owl:Class ;
                                             rdfs:subClassOf <http://purl.obolibrary.org/obo/CRO_0000000> ;
                                             <http://purl.obolibrary.org/obo/IAO_0000115> "Oral presentation intended to present information or teach people about a particular subject, such as a talk or poster presentation at a conference." ;
                                             <http://purl.obolibrary.org/obo/IAO_0000118> "lecture role" ,
                                                                                          "lecturer role" ,
                                                                                          "presentation role" ,
                                                                                          "speaker role" ;
                                             <http://www.geneontology.org/formats/oboInOwl#created_by> <http://orcid.org/0000-0001-5208-3432> ;
                                             rdfs:label "presenter role" .

[ rdf:type owl:Axiom ;
   owl:annotatedSource <http://purl.obolibrary.org/obo/CRO_0000100> ;
   owl:annotatedProperty <http://purl.obolibrary.org/obo/IAO_0000115> ;
   owl:annotatedTarget "Oral presentation intended to present information or teach people about a particular subject, such as a talk or poster presentation at a conference." ;
   <http://purl.obolibrary.org/obo/IAO_0000119> "https://www.wikidata.org/wiki/Q603773"
 ] .


###  http://purl.obolibrary.org/obo/CRO_0000101
<http://purl.obolibrary.org/obo/CRO_0000101> rdf:type owl:Class ;
                                             rdfs:subClassOf <http://purl.obolibrary.org/obo/CRO_0000000> ;
                                             <http://purl.obolibrary.org/obo/IAO_0000115> "Evaluation of scientific, academic, or professional work, such as manuscripts or grants by others working in the same field." ;
                                             <http://purl.obolibrary.org/obo/IAO_0000118> "manuscript review role" ;
                                             <http://www.geneontology.org/formats/oboInOwl#created_by> <http://orcid.org/0000-0001-5208-3432> ;
                                             rdfs:label "peer review role" .

[ rdf:type owl:Axiom ;
   owl:annotatedSource <http://purl.obolibrary.org/obo/CRO_0000101> ;
   owl:annotatedProperty <http://purl.obolibrary.org/obo/IAO_0000115> ;
   owl:annotatedTarget "Evaluation of scientific, academic, or professional work, such as manuscripts or grants by others working in the same field." ;
   <http://purl.obolibrary.org/obo/IAO_0000119> "https://www.lexico.com/en/definition/peer_review"
 ] .


###  http://purl.obolibrary.org/obo/CRO_0000102
<http://purl.obolibrary.org/obo/CRO_0000102> rdf:type owl:Class ;
                                             rdfs:subClassOf <http://purl.obolibrary.org/obo/CRO_0000000> ;
                                             <http://purl.obolibrary.org/obo/IAO_0000115> "A role that involves giving advice in a particular field." ;
                                             <http://purl.obolibrary.org/obo/IAO_0000234> "https://orcid.org/0000-0001-8420-5254" ;
                                             <http://www.geneontology.org/formats/oboInOwl#created_by> <http://orcid.org/0000-0001-5208-3432> ;
                                             rdfs:label "advisory role" .

[ rdf:type owl:Axiom ;
   owl:annotatedSource <http://purl.obolibrary.org/obo/CRO_0000102> ;
   owl:annotatedProperty rdfs:label ;
   owl:annotatedTarget "advisory role" ;
   <http://purl.obolibrary.org/obo/IAO_0000119> "https://www.lexico.com/en/definition/adviser"
 ] .


###  http://purl.obolibrary.org/obo/CRO_0000103
<http://purl.obolibrary.org/obo/CRO_0000103> rdf:type owl:Class ;
                                             rdfs:subClassOf <http://purl.obolibrary.org/obo/CRO_0000000> ;
                                             <http://purl.obolibrary.org/obo/IAO_0000115> "A role that is realized through the modification of an existing artifact (e.g. adding or removing content to/from a document, updating information in a data record, fixing errors in a manuscript, etc.)" ;
                                             <http://purl.obolibrary.org/obo/IAO_0000118> "updater role" ;
                                             <http://purl.obolibrary.org/obo/IAO_0000234> "https://orcid.org/0000-0002-1048-5019" ;
                                             <http://www.geneontology.org/formats/oboInOwl#created_by> <http://orcid.org/0000-0001-5208-3432> ;
                                             rdfs:comment "The nature of a modification will vary depending on the type of artifact being modified, and more specific terms may exist in the CRO to describe certain types of modification." ;
                                             rdfs:label "modifier role" .

[ rdf:type owl:Axiom ;
   owl:annotatedSource <http://purl.obolibrary.org/obo/CRO_0000103> ;
   owl:annotatedProperty <http://purl.obolibrary.org/obo/IAO_0000115> ;
   owl:annotatedTarget "A role that is realized through the modification of an existing artifact (e.g. adding or removing content to/from a document, updating information in a data record, fixing errors in a manuscript, etc.)" ;
   <http://purl.obolibrary.org/obo/IAO_0000119> "https://orcid.org/0000-0002-1048-5019"
 ] .


###  http://purl.obolibrary.org/obo/CRO_0000104
<http://purl.obolibrary.org/obo/CRO_0000104> rdf:type owl:Class ;
                                             rdfs:subClassOf <http://purl.obolibrary.org/obo/CRO_0000000> ;
                                             <http://purl.obolibrary.org/obo/IAO_0000115> "A role that is realized through the act of formally accepting an artifact for inclusion in some larger resource (e.g. database, registry, collection, etc.)" ;
                                             <http://purl.obolibrary.org/obo/IAO_0000234> "https://orcid.org/0000-0002-1048-5019" ;
                                             <http://www.geneontology.org/formats/oboInOwl#created_by> <http://orcid.org/0000-0001-5208-3432> ;
                                             rdfs:comment "An agent accepting an artifact possesses the authority to decide if it belongs in a particular resource or collection. This agent may or may not also have directly evaluated it themselves - but if they did, an 'evaluator role' could additionally be captured." ;
                                             rdfs:label "acceptor role" .

[ rdf:type owl:Axiom ;
   owl:annotatedSource <http://purl.obolibrary.org/obo/CRO_0000104> ;
   owl:annotatedProperty <http://purl.obolibrary.org/obo/IAO_0000115> ;
   owl:annotatedTarget "A role that is realized through the act of formally accepting an artifact for inclusion in some larger resource (e.g. database, registry, collection, etc.)" ;
   <http://purl.obolibrary.org/obo/IAO_0000119> "https://orcid.org/0000-0002-1048-5019"
 ] .


###  http://purl.obolibrary.org/obo/CRO_0000105
<http://purl.obolibrary.org/obo/CRO_0000105> rdf:type owl:Class ;
                                             rdfs:subClassOf <http://purl.obolibrary.org/obo/CRO_0000000> ;
                                             <http://purl.obolibrary.org/obo/IAO_0000115> "A role that is realized through the act of formally submitting or depositing an artifact to be included in some larger resource (e.g. database, registry, collection, etc.)" ;
                                             <http://purl.obolibrary.org/obo/IAO_0000118> "depositor role" ;
                                             <http://purl.obolibrary.org/obo/IAO_0000234> "https://orcid.org/0000-0002-1048-5019" ;
                                             <http://www.geneontology.org/formats/oboInOwl#created_by> <http://orcid.org/0000-0001-5208-3432> ;
                                             rdfs:comment "An agent submitting an artifact may or may not also have contributed to its creation. If they did, and additional ‘creator role’ can be applied." ;
                                             rdfs:label "submitter role" .

[ rdf:type owl:Axiom ;
   owl:annotatedSource <http://purl.obolibrary.org/obo/CRO_0000105> ;
   owl:annotatedProperty <http://purl.obolibrary.org/obo/IAO_0000115> ;
   owl:annotatedTarget "A role that is realized through the act of formally submitting or depositing an artifact to be included in some larger resource (e.g. database, registry, collection, etc.)" ;
   <http://purl.obolibrary.org/obo/IAO_0000119> "https://orcid.org/0000-0002-1048-5019"
 ] .


###  http://purl.obolibrary.org/obo/CRO_0000106
<http://purl.obolibrary.org/obo/CRO_0000106> rdf:type owl:Class ;
                                             rdfs:subClassOf <http://purl.obolibrary.org/obo/CRO_0000078> ;
                                             <http://purl.obolibrary.org/obo/IAO_0000115> "A role that is realized through the review and evaluation of an artifact - generally to assess its quality, completeness, relevance, or other characteristics." ;
                                             <http://purl.obolibrary.org/obo/IAO_0000118> "assessor role" ,
                                                                                          "reviewer role" ;
                                             <http://purl.obolibrary.org/obo/IAO_0000234> "https://orcid.org/0000-0002-1048-5019" ;
                                             <http://www.geneontology.org/formats/oboInOwl#created_by> <http://orcid.org/0000-0001-5208-3432> ;
                                             rdfs:comment "Evaluating an artifact does not involve modification of the assessed artifact - however the suggestion of alterations can be a separate outcome of an evaluation. If the artifact is modified by the agent during or subsequent to the evaluation, a 'modifier role' should additionally be applied." ;
                                             rdfs:label "evaluator role" .

[ rdf:type owl:Axiom ;
   owl:annotatedSource <http://purl.obolibrary.org/obo/CRO_0000106> ;
   owl:annotatedProperty <http://purl.obolibrary.org/obo/IAO_0000115> ;
   owl:annotatedTarget "A role that is realized through the review and evaluation of an artifact - generally to assess its quality, completeness, relevance, or other characteristics." ;
   <http://purl.obolibrary.org/obo/IAO_0000119> "https://orcid.org/0000-0002-1048-5019"
 ] .


###  http://purl.obolibrary.org/obo/CRO_0000107
<http://purl.obolibrary.org/obo/CRO_0000107> rdf:type owl:Class ;
                                             rdfs:subClassOf <http://purl.obolibrary.org/obo/CRO_0000023> ;
                                             <http://purl.obolibrary.org/obo/IAO_0000115> "A role used to indicate that an agent was the creator of an artifact (i.e. had significant or sole responsibility for its initial generation)." ;
                                             <http://purl.obolibrary.org/obo/IAO_0000234> "https://orcid.org/0000-0002-1048-5019" ;
                                             <http://www.geneontology.org/formats/oboInOwl#created_by> <http://orcid.org/0000-0001-5208-3432> ;
                                             rdfs:comment "This is a generic role to be used when a more specific term suitable for the contribution scenario is not available or warranted. For example, the 'author role' term describes creator roles for published works, and should be used to describe creation of things like books or journal articles." ;
                                             rdfs:label "creator role" .

[ rdf:type owl:Axiom ;
   owl:annotatedSource <http://purl.obolibrary.org/obo/CRO_0000107> ;
   owl:annotatedProperty <http://purl.obolibrary.org/obo/IAO_0000115> ;
   owl:annotatedTarget "A role used to indicate that an agent was the creator of an artifact (i.e. had significant or sole responsibility for its initial generation)." ;
   <http://purl.obolibrary.org/obo/IAO_0000119> "https://orcid.org/0000-0002-1048-5019"
 ] .


###  http://purl.obolibrary.org/obo/CRO_0000108
<http://purl.obolibrary.org/obo/CRO_0000108> rdf:type owl:Class ;
                                             rdfs:subClassOf <http://purl.obolibrary.org/obo/CRO_0000015> ;
                                             <http://purl.obolibrary.org/obo/IAO_0000115> "A role that involves creation, maintenance or administration of a database." ;
                                             <http://purl.obolibrary.org/obo/IAO_0000234> "https://orcid.org/0000-0001-8420-5254" ;
                                             <http://www.geneontology.org/formats/oboInOwl#created_by> <http://orcid.org/0000-0001-5208-3432> ;
                                             rdfs:label "database role" .


###  http://purl.obolibrary.org/obo/CRO_0000110
<http://purl.obolibrary.org/obo/CRO_0000110> rdf:type owl:Class ;
                                             rdfs:subClassOf <http://purl.org/credit/ontology#CREDIT_00000005> ;
                                             <http://purl.obolibrary.org/obo/IAO_0000234> "https://orcid.org/0000-0001-8420-5254" ;
                                             <http://www.geneontology.org/formats/oboInOwl#created_by> <http://orcid.org/0000-0001-5208-3432> ;
                                             rdfs:label "community research partner" .


###  http://purl.obolibrary.org/obo/CRO_0000111
<http://purl.obolibrary.org/obo/CRO_0000111> rdf:type owl:Class ;
                                             rdfs:subClassOf <http://purl.obolibrary.org/obo/CRO_0000000> ;
                                             <http://purl.obolibrary.org/obo/IAO_0000115> "A person who deals with provision and maintenance of information in many formats, including: books; electronic resources; magazines; newspapers; audio and video recordings; maps; manuscripts; photographs and other graphic material; bibliographic databases; and web-based and digital resources. A librarian may also provide other information services, including: information literacy instruction; computer provision and training; coordination with community groups to host public programs; assistive technology for people with disabilities; and assistance locating community resources. Librarians often work in a library, but can also work in other physical settings or virtual environments." ;
                                             <http://purl.obolibrary.org/obo/IAO_0000234> "https://orcid.org/0000-0001-8420-5254" ;
                                             <http://www.geneontology.org/formats/oboInOwl#created_by> <http://orcid.org/0000-0001-5208-3432> ;
                                             rdfs:label "librarian role" .

[ rdf:type owl:Axiom ;
   owl:annotatedSource <http://purl.obolibrary.org/obo/CRO_0000111> ;
   owl:annotatedProperty <http://purl.obolibrary.org/obo/IAO_0000115> ;
   owl:annotatedTarget "A person who deals with provision and maintenance of information in many formats, including: books; electronic resources; magazines; newspapers; audio and video recordings; maps; manuscripts; photographs and other graphic material; bibliographic databases; and web-based and digital resources. A librarian may also provide other information services, including: information literacy instruction; computer provision and training; coordination with community groups to host public programs; assistive technology for people with disabilities; and assistance locating community resources. Librarians often work in a library, but can also work in other physical settings or virtual environments." ;
   <http://purl.obolibrary.org/obo/IAO_0000119> "https://en.wikipedia.org/wiki/Librarian"
 ] .


###  http://purl.obolibrary.org/obo/IAO_0000027
<http://purl.obolibrary.org/obo/IAO_0000027> rdfs:subClassOf <http://purl.obolibrary.org/obo/IAO_0000030> .


###  http://purl.obolibrary.org/obo/IAO_0000030
<http://purl.obolibrary.org/obo/IAO_0000030> rdfs:subClassOf <http://purl.obolibrary.org/obo/BFO_0000031> .


###  http://purl.obolibrary.org/obo/IAO_0000078
<http://purl.obolibrary.org/obo/IAO_0000078> rdfs:subClassOf <http://purl.obolibrary.org/obo/IAO_0000102> .


###  http://purl.obolibrary.org/obo/IAO_0000102
<http://purl.obolibrary.org/obo/IAO_0000102> rdfs:subClassOf <http://purl.obolibrary.org/obo/IAO_0000027> .


###  http://purl.obolibrary.org/obo/IAO_0000225
<http://purl.obolibrary.org/obo/IAO_0000225> rdfs:subClassOf <http://purl.obolibrary.org/obo/IAO_0000102> .


###  http://purl.obolibrary.org/obo/IAO_0000409
<http://purl.obolibrary.org/obo/IAO_0000409> rdfs:subClassOf <http://purl.obolibrary.org/obo/IAO_0000102> .


###  http://purl.org/credit/ontology#CREDIT_00000001
<http://purl.org/credit/ontology#CREDIT_00000001> rdf:type owl:Class ;
                                                  rdfs:subClassOf <http://purl.obolibrary.org/obo/CRO_0000000> ;
                                                  <http://purl.obolibrary.org/obo/IAO_0000118> "research conceptualization role" ;
                                                  <http://purl.obolibrary.org/obo/IAO_0000412> "http://purl.org/credit/ontology" .


###  http://purl.org/credit/ontology#CREDIT_00000002
<http://purl.org/credit/ontology#CREDIT_00000002> rdf:type owl:Class ;
                                                  rdfs:subClassOf <http://purl.obolibrary.org/obo/CRO_0000015> ;
                                                  <http://purl.obolibrary.org/obo/IAO_0000412> "http://purl.org/credit/ontology" .


###  http://purl.org/credit/ontology#CREDIT_00000003
<http://purl.org/credit/ontology#CREDIT_00000003> rdf:type owl:Class ;
                                                  rdfs:subClassOf <http://purl.obolibrary.org/obo/CRO_0000000> ;
                                                  <http://purl.obolibrary.org/obo/IAO_0000118> "data analysis role" ;
                                                  <http://purl.obolibrary.org/obo/IAO_0000412> "http://purl.org/credit/ontology" .


###  http://purl.org/credit/ontology#CREDIT_00000004
<http://purl.org/credit/ontology#CREDIT_00000004> rdfs:subClassOf <http://purl.obolibrary.org/obo/CRO_0000000> ;
                                                  <http://purl.obolibrary.org/obo/IAO_0000118> "grant acquisition role" ;
                                                  <http://purl.obolibrary.org/obo/IAO_0000412> "http://purl.org/credit/ontology" .


###  http://purl.org/credit/ontology#CREDIT_00000005
<http://purl.org/credit/ontology#CREDIT_00000005> rdf:type owl:Class ;
                                                  rdfs:subClassOf <http://purl.obolibrary.org/obo/CRO_0000000> ;
                                                  <http://purl.obolibrary.org/obo/IAO_0000412> "http://purl.org/credit/ontology" .


###  http://purl.org/credit/ontology#CREDIT_00000006
<http://purl.org/credit/ontology#CREDIT_00000006> rdf:type owl:Class ;
                                                  rdfs:subClassOf <http://purl.obolibrary.org/obo/CRO_0000000> ;
                                                  <http://purl.obolibrary.org/obo/IAO_0000412> "http://purl.org/credit/ontology" .


###  http://purl.org/credit/ontology#CREDIT_00000007
<http://purl.org/credit/ontology#CREDIT_00000007> rdfs:subClassOf <http://purl.obolibrary.org/obo/CRO_0000000> ;
                                                  <http://purl.obolibrary.org/obo/IAO_0000118> "program administration role" ;
                                                  <http://purl.obolibrary.org/obo/IAO_0000412> "http://purl.org/credit/ontology" .


###  http://purl.org/credit/ontology#CREDIT_00000008
<http://purl.org/credit/ontology#CREDIT_00000008> rdfs:subClassOf <http://purl.obolibrary.org/obo/CRO_0000000> ;
                                                  <http://purl.obolibrary.org/obo/IAO_0000118> "resource provision role" ;
                                                  <http://purl.obolibrary.org/obo/IAO_0000412> "http://purl.org/credit/ontology" .


###  http://purl.org/credit/ontology#CREDIT_00000009
<http://purl.org/credit/ontology#CREDIT_00000009> rdf:type owl:Class ;
                                                  rdfs:subClassOf <http://purl.obolibrary.org/obo/CRO_0000000> ;
                                                  <http://purl.obolibrary.org/obo/IAO_0000118> "software systems role" ;
                                                  <http://purl.obolibrary.org/obo/IAO_0000412> "http://purl.org/credit/ontology" .


###  http://purl.org/credit/ontology#CREDIT_00000010
<http://purl.org/credit/ontology#CREDIT_00000010> rdfs:subClassOf <http://purl.obolibrary.org/obo/CRO_0000000> ;
                                                  <http://purl.obolibrary.org/obo/IAO_0000118> "supervisory role" ;
                                                  <http://purl.obolibrary.org/obo/IAO_0000412> "http://purl.org/credit/ontology" .


###  http://purl.org/credit/ontology#CREDIT_00000011
<http://purl.org/credit/ontology#CREDIT_00000011> rdfs:subClassOf <http://purl.obolibrary.org/obo/CRO_0000000> ;
                                                  <http://purl.obolibrary.org/obo/IAO_0000412> "http://purl.org/credit/ontology" .


###  http://purl.org/credit/ontology#CREDIT_00000012
<http://purl.org/credit/ontology#CREDIT_00000012> rdfs:subClassOf <http://purl.obolibrary.org/obo/CRO_0000000> ;
                                                  <http://purl.obolibrary.org/obo/IAO_0000412> "http://purl.org/credit/ontology" .


###  http://purl.org/credit/ontology#CREDIT_00000013
<http://purl.org/credit/ontology#CREDIT_00000013> rdf:type owl:Class ;
                                                  rdfs:subClassOf <http://purl.obolibrary.org/obo/CRO_0000001> ;
                                                  <http://purl.obolibrary.org/obo/IAO_0000118> "original draft preparation role" ;
                                                  <http://purl.obolibrary.org/obo/IAO_0000412> "http://purl.org/credit/ontology" .


###  http://purl.org/credit/ontology#CREDIT_00000014
<http://purl.org/credit/ontology#CREDIT_00000014> rdfs:subClassOf <http://purl.obolibrary.org/obo/CRO_0000001> ;
                                                  <http://purl.obolibrary.org/obo/IAO_0000412> "http://purl.org/credit/ontology" .


###  http://www.geneontology.org/formats/oboInOwl#Subset
<http://www.geneontology.org/formats/oboInOwl#Subset> rdfs:subClassOf <http://purl.obolibrary.org/obo/IAO_0000102> .


###  Generated by the OWL API (version 1.1.0) https://github.com/owlcs/owlapi
